<?xml version="1.0"?>
<rdf:RDF xmlns="http://www.semanticweb.org/patriciapoveda/ontologies/2020/4/ontology-place"
     xml:base="http://www.semanticweb.org/patriciapoveda/ontologies/2020/4/ontology-place"
     xmlns:owl="http://www.w3.org/2002/07/owl#"
     xmlns:rdf="http://www.w3.org/1999/02/22-rdf-syntax-ns#"
     xmlns:xml="http://www.w3.org/XML/1998/namespace"
     xmlns:xsd="http://www.w3.org/2001/XMLSchema#"
     xmlns:rdfs="http://www.w3.org/2000/01/rdf-schema#"
     xmlns:place="http://www.ontologydesignpatterns.org/cp/owl/place.owl#"
     xmlns:ontologia="https://apiict01.etsii.upm.es/mediawiki/index.php/User:PatriciaPoveda/ontologia.owl#"
     xmlns:timeinterval="http://www.ontologydesignpatterns.org/cp/owl/timeinterval.owl#"
     xmlns:ontology-place="http://www.semanticweb.org/patriciapoveda/ontologies/2020/4/ontology-place.owl#"
     xmlns:cpannotationschema="http://www.ontologydesignpatterns.org/schemas/cpannotationschema.owl#">
    <owl:Ontology rdf:about="http://www.semanticweb.org/patriciapoveda/ontologies/2020/4/ontology-place.owl">
        <owl:imports rdf:resource="http://www.ontologydesignpatterns.org/schemas/cpannotationschema.owl"/>
        <ontologia:Autor>Patricia Poveda Hernández</ontologia:Autor>
        <ontologia:Año rdf:datatype="http://www.w3.org/2001/XMLSchema#integer">2020</ontologia:Año>
        <ontologia:Descripción xml:lang="es">Desarrollo de una ontología para entender y controlar la información que forma parte de un sistema de transporte encargado de la recogida de materiales metálicos, obtenidos del cliente por parte del proveedor para su posterior reutilización.</ontologia:Descripción>
        <ontologia:Titulo>Logística inversa en Control de flotas</ontologia:Titulo>
        <ontologia:Tutor>Joaquín Ordieres Meré</ontologia:Tutor>
    </owl:Ontology>
    


    <!-- 
    ///////////////////////////////////////////////////////////////////////////////////////
    //
    // Annotation properties
    //
    ///////////////////////////////////////////////////////////////////////////////////////
     -->

    


    <!-- http://www.ontologydesignpatterns.org/schemas/cpannotationschema.owl#coversRequirements -->

    <owl:AnnotationProperty rdf:about="http://www.ontologydesignpatterns.org/schemas/cpannotationschema.owl#coversRequirements"/>
    


    <!-- http://www.ontologydesignpatterns.org/schemas/cpannotationschema.owl#extractedFrom -->

    <owl:AnnotationProperty rdf:about="http://www.ontologydesignpatterns.org/schemas/cpannotationschema.owl#extractedFrom"/>
    


    <!-- http://www.ontologydesignpatterns.org/schemas/cpannotationschema.owl#hasAuthor -->

    <owl:AnnotationProperty rdf:about="http://www.ontologydesignpatterns.org/schemas/cpannotationschema.owl#hasAuthor"/>
    


    <!-- http://www.ontologydesignpatterns.org/schemas/cpannotationschema.owl#hasConsequences -->

    <owl:AnnotationProperty rdf:about="http://www.ontologydesignpatterns.org/schemas/cpannotationschema.owl#hasConsequences"/>
    


    <!-- http://www.ontologydesignpatterns.org/schemas/cpannotationschema.owl#hasIntent -->

    <owl:AnnotationProperty rdf:about="http://www.ontologydesignpatterns.org/schemas/cpannotationschema.owl#hasIntent"/>
    


    <!-- http://www.ontologydesignpatterns.org/schemas/cpannotationschema.owl#relatedCPs -->

    <owl:AnnotationProperty rdf:about="http://www.ontologydesignpatterns.org/schemas/cpannotationschema.owl#relatedCPs"/>
    


    <!-- http://www.ontologydesignpatterns.org/schemas/cpannotationschema.owl#scenarios -->

    <owl:AnnotationProperty rdf:about="http://www.ontologydesignpatterns.org/schemas/cpannotationschema.owl#scenarios"/>
    


    <!-- http://www.w3.org/2000/01/rdf-schema#comment -->

    <owl:AnnotationProperty rdf:about="http://www.w3.org/2000/01/rdf-schema#comment"/>
    


    <!-- http://www.w3.org/2000/01/rdf-schema#isDefinedBy -->

    <owl:AnnotationProperty rdf:about="http://www.w3.org/2000/01/rdf-schema#isDefinedBy"/>
    


    <!-- http://www.w3.org/2000/01/rdf-schema#label -->

    <owl:AnnotationProperty rdf:about="http://www.w3.org/2000/01/rdf-schema#label"/>
    


    <!-- http://www.w3.org/2002/07/owl#versionInfo -->

    <owl:AnnotationProperty rdf:about="http://www.w3.org/2002/07/owl#versionInfo"/>
    


    <!-- https://apiict01.etsii.upm.es/mediawiki/index.php/User:PatriciaPoveda/ontologia.owl#Autor -->

    <owl:AnnotationProperty rdf:about="https://apiict01.etsii.upm.es/mediawiki/index.php/User:PatriciaPoveda/ontologia.owl#Autor">
        <rdfs:subPropertyOf rdf:resource="http://www.w3.org/2000/01/rdf-schema#label"/>
    </owl:AnnotationProperty>
    


    <!-- https://apiict01.etsii.upm.es/mediawiki/index.php/User:PatriciaPoveda/ontologia.owl#Año -->

    <owl:AnnotationProperty rdf:about="https://apiict01.etsii.upm.es/mediawiki/index.php/User:PatriciaPoveda/ontologia.owl#Año">
        <rdfs:subPropertyOf rdf:resource="http://www.w3.org/2000/01/rdf-schema#label"/>
    </owl:AnnotationProperty>
    


    <!-- https://apiict01.etsii.upm.es/mediawiki/index.php/User:PatriciaPoveda/ontologia.owl#Descripción -->

    <owl:AnnotationProperty rdf:about="https://apiict01.etsii.upm.es/mediawiki/index.php/User:PatriciaPoveda/ontologia.owl#Descripción">
        <rdfs:subPropertyOf rdf:resource="http://www.w3.org/2000/01/rdf-schema#label"/>
    </owl:AnnotationProperty>
    


    <!-- https://apiict01.etsii.upm.es/mediawiki/index.php/User:PatriciaPoveda/ontologia.owl#Titulo -->

    <owl:AnnotationProperty rdf:about="https://apiict01.etsii.upm.es/mediawiki/index.php/User:PatriciaPoveda/ontologia.owl#Titulo">
        <rdfs:subPropertyOf rdf:resource="http://www.w3.org/2000/01/rdf-schema#label"/>
    </owl:AnnotationProperty>
    


    <!-- https://apiict01.etsii.upm.es/mediawiki/index.php/User:PatriciaPoveda/ontologia.owl#Tutor -->

    <owl:AnnotationProperty rdf:about="https://apiict01.etsii.upm.es/mediawiki/index.php/User:PatriciaPoveda/ontologia.owl#Tutor">
        <rdfs:subPropertyOf rdf:resource="http://www.w3.org/2000/01/rdf-schema#label"/>
    </owl:AnnotationProperty>
    


    <!-- 
    ///////////////////////////////////////////////////////////////////////////////////////
    //
    // Object Properties
    //
    ///////////////////////////////////////////////////////////////////////////////////////
     -->

    


    <!-- http://www.ontologydesignpatterns.org/cp/owl/place.owl#isLocationOf -->

    <owl:ObjectProperty rdf:about="http://www.ontologydesignpatterns.org/cp/owl/place.owl#isLocationOf">
        <rdf:type rdf:resource="http://www.w3.org/2002/07/owl#TransitiveProperty"/>
        <rdfs:comment>A generic, relative localization, holding between any entities. E.g. &apos;Rome is the seat of the Pope&apos;, &apos;the liver is the location of the tumor&apos;.
As a very general notion of localization, it is assumed as transitive.
For &apos;absolute&apos; locations, see SpaceRegion</rdfs:comment>
        <rdfs:isDefinedBy rdf:resource="http://www.ontologydesignpatterns.org/cp/owl/place.owl"/>
        <rdfs:label xml:lang="en">is location of</rdfs:label>
    </owl:ObjectProperty>
    


    <!-- http://www.ontologydesignpatterns.org/cp/owl/place.owl#is_located_in -->

    <owl:ObjectProperty rdf:about="http://www.ontologydesignpatterns.org/cp/owl/place.owl#is_located_in">
        <rdf:type rdf:resource="http://www.w3.org/2002/07/owl#TransitiveProperty"/>
        <rdfs:comment>A generic, relative localization, holding between any entities. E.g. &apos;the cat is on the mat&apos;, &apos;Omar is in Samarcanda&apos;, &apos;the wound is close to the femural artery&apos;.
For &apos;absolute&apos; locations, see SpaceRegion</rdfs:comment>
        <rdfs:isDefinedBy rdf:resource="http://www.ontologydesignpatterns.org/cp/owl/place.owl"/>
        <rdfs:label xml:lang="en">is located in</rdfs:label>
    </owl:ObjectProperty>
    


    <!-- http://www.semanticweb.org/patriciapoveda/ontologies/2020/4/ontology-place.owl#are_divided_by -->

    <owl:ObjectProperty rdf:about="http://www.semanticweb.org/patriciapoveda/ontologies/2020/4/ontology-place.owl#are_divided_by">
        <owl:inverseOf rdf:resource="http://www.semanticweb.org/patriciapoveda/ontologies/2020/4/ontology-place.owl#divide"/>
        <rdfs:domain rdf:resource="https://apiict01.etsii.upm.es/mediawiki/index.php/User:PatriciaPoveda/ontologia.owl#Segments"/>
        <rdfs:range rdf:resource="https://apiict01.etsii.upm.es/mediawiki/index.php/User:PatriciaPoveda/ontologia.owl#Stops_Inter-segment"/>
    </owl:ObjectProperty>
    


    <!-- http://www.semanticweb.org/patriciapoveda/ontologies/2020/4/ontology-place.owl#are_opened_hours -->

    <owl:ObjectProperty rdf:about="http://www.semanticweb.org/patriciapoveda/ontologies/2020/4/ontology-place.owl#are_opened_hours">
        <owl:inverseOf rdf:resource="http://www.semanticweb.org/patriciapoveda/ontologies/2020/4/ontology-place.owl#has_opening_hours"/>
        <rdfs:domain rdf:resource="http://www.ontologydesignpatterns.org/cp/owl/timeinterval.owl#TimeInterval"/>
        <rdfs:range rdf:resource="https://apiict01.etsii.upm.es/mediawiki/index.php/User:PatriciaPoveda/ontologia.owl#Warehouses"/>
    </owl:ObjectProperty>
    


    <!-- http://www.semanticweb.org/patriciapoveda/ontologies/2020/4/ontology-place.owl#divide -->

    <owl:ObjectProperty rdf:about="http://www.semanticweb.org/patriciapoveda/ontologies/2020/4/ontology-place.owl#divide">
        <rdfs:domain rdf:resource="https://apiict01.etsii.upm.es/mediawiki/index.php/User:PatriciaPoveda/ontologia.owl#Stops_Inter-segment"/>
        <rdfs:range rdf:resource="https://apiict01.etsii.upm.es/mediawiki/index.php/User:PatriciaPoveda/ontologia.owl#Segments"/>
    </owl:ObjectProperty>
    


    <!-- http://www.semanticweb.org/patriciapoveda/ontologies/2020/4/ontology-place.owl#form -->

    <owl:ObjectProperty rdf:about="http://www.semanticweb.org/patriciapoveda/ontologies/2020/4/ontology-place.owl#form">
        <owl:inverseOf rdf:resource="http://www.semanticweb.org/patriciapoveda/ontologies/2020/4/ontology-place.owl#is_formed_by"/>
        <rdfs:domain rdf:resource="https://apiict01.etsii.upm.es/mediawiki/index.php/User:PatriciaPoveda/ontologia.owl#Segments"/>
        <rdfs:range rdf:resource="https://apiict01.etsii.upm.es/mediawiki/index.php/User:PatriciaPoveda/ontologia.owl#Trajectory"/>
    </owl:ObjectProperty>
    


    <!-- http://www.semanticweb.org/patriciapoveda/ontologies/2020/4/ontology-place.owl#gives_first_weight -->

    <owl:ObjectProperty rdf:about="http://www.semanticweb.org/patriciapoveda/ontologies/2020/4/ontology-place.owl#gives_first_weight">
        <owl:inverseOf rdf:resource="http://www.semanticweb.org/patriciapoveda/ontologies/2020/4/ontology-place.owl#is_first_weight_given_by"/>
        <rdfs:domain rdf:resource="http://www.semanticweb.org/patriciapoveda/ontologies/2020/4/ontology-place.owl#Cust.Weighing_Worker"/>
        <rdfs:range rdf:resource="http://www.semanticweb.org/patriciapoveda/ontologies/2020/4/ontology-place.owl#Customer_Scale"/>
    </owl:ObjectProperty>
    


    <!-- http://www.semanticweb.org/patriciapoveda/ontologies/2020/4/ontology-place.owl#gives_second_weight -->

    <owl:ObjectProperty rdf:about="http://www.semanticweb.org/patriciapoveda/ontologies/2020/4/ontology-place.owl#gives_second_weight">
        <owl:inverseOf rdf:resource="http://www.semanticweb.org/patriciapoveda/ontologies/2020/4/ontology-place.owl#is_second_weight_given_by"/>
        <rdfs:domain rdf:resource="http://www.semanticweb.org/patriciapoveda/ontologies/2020/4/ontology-place.owl#Sup.Weighing_Worker"/>
        <rdfs:range rdf:resource="http://www.semanticweb.org/patriciapoveda/ontologies/2020/4/ontology-place.owl#Warehouse_Scale"/>
    </owl:ObjectProperty>
    


    <!-- http://www.semanticweb.org/patriciapoveda/ontologies/2020/4/ontology-place.owl#happen_in -->

    <owl:ObjectProperty rdf:about="http://www.semanticweb.org/patriciapoveda/ontologies/2020/4/ontology-place.owl#happen_in">
        <owl:inverseOf rdf:resource="http://www.semanticweb.org/patriciapoveda/ontologies/2020/4/ontology-place.owl#has"/>
        <rdfs:domain rdf:resource="https://apiict01.etsii.upm.es/mediawiki/index.php/User:PatriciaPoveda/ontologia.owl#Stops_Inter-segment"/>
        <rdfs:range rdf:resource="https://apiict01.etsii.upm.es/mediawiki/index.php/User:PatriciaPoveda/ontologia.owl#Trajectory"/>
    </owl:ObjectProperty>
    


    <!-- http://www.semanticweb.org/patriciapoveda/ontologies/2020/4/ontology-place.owl#has -->

    <owl:ObjectProperty rdf:about="http://www.semanticweb.org/patriciapoveda/ontologies/2020/4/ontology-place.owl#has">
        <rdfs:domain rdf:resource="https://apiict01.etsii.upm.es/mediawiki/index.php/User:PatriciaPoveda/ontologia.owl#Trajectory"/>
        <rdfs:range rdf:resource="https://apiict01.etsii.upm.es/mediawiki/index.php/User:PatriciaPoveda/ontologia.owl#Stops_Inter-segment"/>
    </owl:ObjectProperty>
    


    <!-- http://www.semanticweb.org/patriciapoveda/ontologies/2020/4/ontology-place.owl#has_as_destination -->

    <owl:ObjectProperty rdf:about="http://www.semanticweb.org/patriciapoveda/ontologies/2020/4/ontology-place.owl#has_as_destination">
        <owl:inverseOf rdf:resource="http://www.semanticweb.org/patriciapoveda/ontologies/2020/4/ontology-place.owl#is_destination_of"/>
        <rdfs:domain rdf:resource="https://apiict01.etsii.upm.es/mediawiki/index.php/User:PatriciaPoveda/ontologia.owl#Trajectory"/>
        <rdfs:range rdf:resource="http://www.semanticweb.org/patriciapoveda/ontologies/2020/4/ontology-place.owl#Product_Warehouse"/>
    </owl:ObjectProperty>
    


    <!-- http://www.semanticweb.org/patriciapoveda/ontologies/2020/4/ontology-place.owl#has_end_point_in -->

    <owl:ObjectProperty rdf:about="http://www.semanticweb.org/patriciapoveda/ontologies/2020/4/ontology-place.owl#has_end_point_in">
        <owl:inverseOf rdf:resource="http://www.semanticweb.org/patriciapoveda/ontologies/2020/4/ontology-place.owl#is_ended_point_of"/>
        <rdfs:domain rdf:resource="https://apiict01.etsii.upm.es/mediawiki/index.php/User:PatriciaPoveda/ontologia.owl#Trajectory"/>
        <rdfs:range rdf:resource="http://www.semanticweb.org/patriciapoveda/ontologies/2020/4/ontology-place.owl#Vehicle_Garage"/>
        <rdfs:label>has end point in</rdfs:label>
    </owl:ObjectProperty>
    


    <!-- http://www.semanticweb.org/patriciapoveda/ontologies/2020/4/ontology-place.owl#has_opening_hours -->

    <owl:ObjectProperty rdf:about="http://www.semanticweb.org/patriciapoveda/ontologies/2020/4/ontology-place.owl#has_opening_hours">
        <rdfs:domain rdf:resource="https://apiict01.etsii.upm.es/mediawiki/index.php/User:PatriciaPoveda/ontologia.owl#Warehouses"/>
        <rdfs:range rdf:resource="http://www.ontologydesignpatterns.org/cp/owl/timeinterval.owl#TimeInterval"/>
    </owl:ObjectProperty>
    


    <!-- http://www.semanticweb.org/patriciapoveda/ontologies/2020/4/ontology-place.owl#has_order_and_expiration_date -->

    <owl:ObjectProperty rdf:about="http://www.semanticweb.org/patriciapoveda/ontologies/2020/4/ontology-place.owl#has_order_and_expiration_date">
        <owl:inverseOf rdf:resource="http://www.semanticweb.org/patriciapoveda/ontologies/2020/4/ontology-place.owl#is_order/expiration_date_of"/>
        <rdfs:domain rdf:resource="https://apiict01.etsii.upm.es/mediawiki/index.php/User:PatriciaPoveda/ontologia.owl#Product"/>
        <rdfs:range rdf:resource="http://www.ontologydesignpatterns.org/cp/owl/timeinterval.owl#TimeInterval"/>
    </owl:ObjectProperty>
    


    <!-- http://www.semanticweb.org/patriciapoveda/ontologies/2020/4/ontology-place.owl#has_start_point_in -->

    <owl:ObjectProperty rdf:about="http://www.semanticweb.org/patriciapoveda/ontologies/2020/4/ontology-place.owl#has_start_point_in">
        <owl:inverseOf rdf:resource="http://www.semanticweb.org/patriciapoveda/ontologies/2020/4/ontology-place.owl#is_started_point_of"/>
        <rdfs:domain rdf:resource="https://apiict01.etsii.upm.es/mediawiki/index.php/User:PatriciaPoveda/ontologia.owl#Trajectory"/>
        <rdfs:range rdf:resource="http://www.semanticweb.org/patriciapoveda/ontologies/2020/4/ontology-place.owl#Vehicle_Garage"/>
        <rdfs:label>has start point in</rdfs:label>
    </owl:ObjectProperty>
    


    <!-- http://www.semanticweb.org/patriciapoveda/ontologies/2020/4/ontology-place.owl#has_time_slot -->

    <owl:ObjectProperty rdf:about="http://www.semanticweb.org/patriciapoveda/ontologies/2020/4/ontology-place.owl#has_time_slot">
        <owl:inverseOf rdf:resource="http://www.semanticweb.org/patriciapoveda/ontologies/2020/4/ontology-place.owl#is_time_slot"/>
        <rdfs:domain rdf:resource="https://apiict01.etsii.upm.es/mediawiki/index.php/User:PatriciaPoveda/ontologia.owl#Customer"/>
        <rdfs:range rdf:resource="http://www.ontologydesignpatterns.org/cp/owl/timeinterval.owl#TimeInterval"/>
    </owl:ObjectProperty>
    


    <!-- http://www.semanticweb.org/patriciapoveda/ontologies/2020/4/ontology-place.owl#has_working_hours -->

    <owl:ObjectProperty rdf:about="http://www.semanticweb.org/patriciapoveda/ontologies/2020/4/ontology-place.owl#has_working_hours">
        <owl:inverseOf rdf:resource="http://www.semanticweb.org/patriciapoveda/ontologies/2020/4/ontology-place.owl#is_working_shcedule_of"/>
        <rdfs:domain rdf:resource="http://www.semanticweb.org/patriciapoveda/ontologies/2020/4/ontology-place.owl#Supplier"/>
        <rdfs:range rdf:resource="http://www.ontologydesignpatterns.org/cp/owl/timeinterval.owl#TimeInterval"/>
    </owl:ObjectProperty>
    


    <!-- http://www.semanticweb.org/patriciapoveda/ontologies/2020/4/ontology-place.owl#includes -->

    <owl:ObjectProperty rdf:about="http://www.semanticweb.org/patriciapoveda/ontologies/2020/4/ontology-place.owl#includes">
        <owl:inverseOf rdf:resource="http://www.semanticweb.org/patriciapoveda/ontologies/2020/4/ontology-place.owl#is_included"/>
        <rdfs:domain rdf:resource="https://apiict01.etsii.upm.es/mediawiki/index.php/User:PatriciaPoveda/ontologia.owl#Trajectory"/>
        <rdfs:range rdf:resource="https://apiict01.etsii.upm.es/mediawiki/index.php/User:PatriciaPoveda/ontologia.owl#Customer"/>
        <rdfs:label>includes</rdfs:label>
    </owl:ObjectProperty>
    


    <!-- http://www.semanticweb.org/patriciapoveda/ontologies/2020/4/ontology-place.owl#is_destination_of -->

    <owl:ObjectProperty rdf:about="http://www.semanticweb.org/patriciapoveda/ontologies/2020/4/ontology-place.owl#is_destination_of">
        <rdfs:domain rdf:resource="http://www.semanticweb.org/patriciapoveda/ontologies/2020/4/ontology-place.owl#Product_Warehouse"/>
        <rdfs:range rdf:resource="https://apiict01.etsii.upm.es/mediawiki/index.php/User:PatriciaPoveda/ontologia.owl#Trajectory"/>
    </owl:ObjectProperty>
    


    <!-- http://www.semanticweb.org/patriciapoveda/ontologies/2020/4/ontology-place.owl#is_duration__of -->

    <owl:ObjectProperty rdf:about="http://www.semanticweb.org/patriciapoveda/ontologies/2020/4/ontology-place.owl#is_duration__of">
        <owl:inverseOf rdf:resource="http://www.semanticweb.org/patriciapoveda/ontologies/2020/4/ontology-place.owl#last"/>
        <rdfs:domain rdf:resource="http://www.ontologydesignpatterns.org/cp/owl/timeinterval.owl#TimeInterval"/>
        <rdfs:range rdf:resource="https://apiict01.etsii.upm.es/mediawiki/index.php/User:PatriciaPoveda/ontologia.owl#Stops_Inter-segment"/>
    </owl:ObjectProperty>
    


    <!-- http://www.semanticweb.org/patriciapoveda/ontologies/2020/4/ontology-place.owl#is_ended_point_of -->

    <owl:ObjectProperty rdf:about="http://www.semanticweb.org/patriciapoveda/ontologies/2020/4/ontology-place.owl#is_ended_point_of">
        <rdfs:domain rdf:resource="http://www.semanticweb.org/patriciapoveda/ontologies/2020/4/ontology-place.owl#Vehicle_Garage"/>
        <rdfs:range rdf:resource="https://apiict01.etsii.upm.es/mediawiki/index.php/User:PatriciaPoveda/ontologia.owl#Trajectory"/>
        <rdfs:label>is end point of</rdfs:label>
    </owl:ObjectProperty>
    


    <!-- http://www.semanticweb.org/patriciapoveda/ontologies/2020/4/ontology-place.owl#is_first_weight_given_by -->

    <owl:ObjectProperty rdf:about="http://www.semanticweb.org/patriciapoveda/ontologies/2020/4/ontology-place.owl#is_first_weight_given_by">
        <rdfs:domain rdf:resource="http://www.semanticweb.org/patriciapoveda/ontologies/2020/4/ontology-place.owl#Customer_Scale"/>
        <rdfs:range rdf:resource="http://www.semanticweb.org/patriciapoveda/ontologies/2020/4/ontology-place.owl#Cust.Weighing_Worker"/>
    </owl:ObjectProperty>
    


    <!-- http://www.semanticweb.org/patriciapoveda/ontologies/2020/4/ontology-place.owl#is_formed_by -->

    <owl:ObjectProperty rdf:about="http://www.semanticweb.org/patriciapoveda/ontologies/2020/4/ontology-place.owl#is_formed_by">
        <rdfs:domain rdf:resource="https://apiict01.etsii.upm.es/mediawiki/index.php/User:PatriciaPoveda/ontologia.owl#Trajectory"/>
        <rdfs:range rdf:resource="https://apiict01.etsii.upm.es/mediawiki/index.php/User:PatriciaPoveda/ontologia.owl#Segments"/>
    </owl:ObjectProperty>
    


    <!-- http://www.semanticweb.org/patriciapoveda/ontologies/2020/4/ontology-place.owl#is_in_position -->

    <owl:ObjectProperty rdf:about="http://www.semanticweb.org/patriciapoveda/ontologies/2020/4/ontology-place.owl#is_in_position">
        <owl:inverseOf rdf:resource="http://www.semanticweb.org/patriciapoveda/ontologies/2020/4/ontology-place.owl#is_position_of"/>
        <rdfs:domain rdf:resource="http://www.semanticweb.org/patriciapoveda/ontologies/2020/4/ontology-place.owl#Download"/>
        <rdfs:domain rdf:resource="https://apiict01.etsii.upm.es/mediawiki/index.php/User:PatriciaPoveda/ontologia.owl#Agents"/>
        <rdfs:domain rdf:resource="https://apiict01.etsii.upm.es/mediawiki/index.php/User:PatriciaPoveda/ontologia.owl#Stops_Inter-segment"/>
        <rdfs:domain rdf:resource="https://apiict01.etsii.upm.es/mediawiki/index.php/User:PatriciaPoveda/ontologia.owl#Vehicle"/>
        <rdfs:range rdf:resource="http://www.semanticweb.org/patriciapoveda/ontologies/2020/4/ontology-place.owl#Real_Time_Location"/>
    </owl:ObjectProperty>
    


    <!-- http://www.semanticweb.org/patriciapoveda/ontologies/2020/4/ontology-place.owl#is_in_stage -->

    <owl:ObjectProperty rdf:about="http://www.semanticweb.org/patriciapoveda/ontologies/2020/4/ontology-place.owl#is_in_stage">
        <owl:inverseOf rdf:resource="http://www.semanticweb.org/patriciapoveda/ontologies/2020/4/ontology-place.owl#is_stage_of"/>
        <rdf:type rdf:resource="http://www.w3.org/2002/07/owl#SymmetricProperty"/>
        <rdfs:domain rdf:resource="http://www.semanticweb.org/patriciapoveda/ontologies/2020/4/ontology-place.owl#Supplier"/>
        <rdfs:domain rdf:resource="https://apiict01.etsii.upm.es/mediawiki/index.php/User:PatriciaPoveda/ontologia.owl#Product"/>
        <rdfs:range rdf:resource="http://www.semanticweb.org/patriciapoveda/ontologies/2020/4/ontology-place.owl#Activities"/>
    </owl:ObjectProperty>
    


    <!-- http://www.semanticweb.org/patriciapoveda/ontologies/2020/4/ontology-place.owl#is_included -->

    <owl:ObjectProperty rdf:about="http://www.semanticweb.org/patriciapoveda/ontologies/2020/4/ontology-place.owl#is_included">
        <rdfs:domain rdf:resource="https://apiict01.etsii.upm.es/mediawiki/index.php/User:PatriciaPoveda/ontologia.owl#Customer"/>
        <rdfs:range rdf:resource="https://apiict01.etsii.upm.es/mediawiki/index.php/User:PatriciaPoveda/ontologia.owl#Trajectory"/>
        <rdfs:label>is included in</rdfs:label>
    </owl:ObjectProperty>
    


    <!-- http://www.semanticweb.org/patriciapoveda/ontologies/2020/4/ontology-place.owl#is_parked_in -->

    <owl:ObjectProperty rdf:about="http://www.semanticweb.org/patriciapoveda/ontologies/2020/4/ontology-place.owl#is_parked_in">
        <owl:inverseOf rdf:resource="http://www.semanticweb.org/patriciapoveda/ontologies/2020/4/ontology-place.owl#is_the_park_of"/>
        <rdfs:domain rdf:resource="https://apiict01.etsii.upm.es/mediawiki/index.php/User:PatriciaPoveda/ontologia.owl#Vehicle"/>
        <rdfs:range rdf:resource="http://www.semanticweb.org/patriciapoveda/ontologies/2020/4/ontology-place.owl#Vehicle_Garage"/>
        <rdfs:label>is parked in</rdfs:label>
    </owl:ObjectProperty>
    


    <!-- http://www.semanticweb.org/patriciapoveda/ontologies/2020/4/ontology-place.owl#is_position_of -->

    <owl:ObjectProperty rdf:about="http://www.semanticweb.org/patriciapoveda/ontologies/2020/4/ontology-place.owl#is_position_of">
        <rdfs:domain rdf:resource="http://www.semanticweb.org/patriciapoveda/ontologies/2020/4/ontology-place.owl#Real_Time_Location"/>
        <rdfs:range rdf:resource="http://www.semanticweb.org/patriciapoveda/ontologies/2020/4/ontology-place.owl#Download"/>
        <rdfs:range rdf:resource="https://apiict01.etsii.upm.es/mediawiki/index.php/User:PatriciaPoveda/ontologia.owl#Agents"/>
        <rdfs:range rdf:resource="https://apiict01.etsii.upm.es/mediawiki/index.php/User:PatriciaPoveda/ontologia.owl#Stops_Inter-segment"/>
        <rdfs:range rdf:resource="https://apiict01.etsii.upm.es/mediawiki/index.php/User:PatriciaPoveda/ontologia.owl#Vehicle"/>
    </owl:ObjectProperty>
    


    <!-- http://www.semanticweb.org/patriciapoveda/ontologies/2020/4/ontology-place.owl#is_second_weight_given_by -->

    <owl:ObjectProperty rdf:about="http://www.semanticweb.org/patriciapoveda/ontologies/2020/4/ontology-place.owl#is_second_weight_given_by">
        <rdfs:domain rdf:resource="http://www.semanticweb.org/patriciapoveda/ontologies/2020/4/ontology-place.owl#Warehouse_Scale"/>
        <rdfs:range rdf:resource="http://www.semanticweb.org/patriciapoveda/ontologies/2020/4/ontology-place.owl#Sup.Weighing_Worker"/>
    </owl:ObjectProperty>
    


    <!-- http://www.semanticweb.org/patriciapoveda/ontologies/2020/4/ontology-place.owl#is_stage_of -->

    <owl:ObjectProperty rdf:about="http://www.semanticweb.org/patriciapoveda/ontologies/2020/4/ontology-place.owl#is_stage_of">
        <rdfs:domain rdf:resource="http://www.semanticweb.org/patriciapoveda/ontologies/2020/4/ontology-place.owl#Activities"/>
        <rdfs:range rdf:resource="http://www.semanticweb.org/patriciapoveda/ontologies/2020/4/ontology-place.owl#Supplier"/>
        <rdfs:range rdf:resource="https://apiict01.etsii.upm.es/mediawiki/index.php/User:PatriciaPoveda/ontologia.owl#Product"/>
    </owl:ObjectProperty>
    


    <!-- http://www.semanticweb.org/patriciapoveda/ontologies/2020/4/ontology-place.owl#is_started_point_of -->

    <owl:ObjectProperty rdf:about="http://www.semanticweb.org/patriciapoveda/ontologies/2020/4/ontology-place.owl#is_started_point_of">
        <rdfs:domain rdf:resource="http://www.semanticweb.org/patriciapoveda/ontologies/2020/4/ontology-place.owl#Vehicle_Garage"/>
        <rdfs:range rdf:resource="https://apiict01.etsii.upm.es/mediawiki/index.php/User:PatriciaPoveda/ontologia.owl#Trajectory"/>
        <rdfs:label>is starting point of</rdfs:label>
    </owl:ObjectProperty>
    


    <!-- http://www.semanticweb.org/patriciapoveda/ontologies/2020/4/ontology-place.owl#is_the_park_of -->

    <owl:ObjectProperty rdf:about="http://www.semanticweb.org/patriciapoveda/ontologies/2020/4/ontology-place.owl#is_the_park_of">
        <rdfs:domain rdf:resource="http://www.semanticweb.org/patriciapoveda/ontologies/2020/4/ontology-place.owl#Vehicle_Garage"/>
        <rdfs:range rdf:resource="https://apiict01.etsii.upm.es/mediawiki/index.php/User:PatriciaPoveda/ontologia.owl#Vehicle"/>
        <rdfs:label>is the parking of</rdfs:label>
    </owl:ObjectProperty>
    


    <!-- http://www.semanticweb.org/patriciapoveda/ontologies/2020/4/ontology-place.owl#is_time_slot -->

    <owl:ObjectProperty rdf:about="http://www.semanticweb.org/patriciapoveda/ontologies/2020/4/ontology-place.owl#is_time_slot">
        <rdfs:domain rdf:resource="http://www.ontologydesignpatterns.org/cp/owl/timeinterval.owl#TimeInterval"/>
        <rdfs:range rdf:resource="https://apiict01.etsii.upm.es/mediawiki/index.php/User:PatriciaPoveda/ontologia.owl#Customer"/>
    </owl:ObjectProperty>
    


    <!-- http://www.semanticweb.org/patriciapoveda/ontologies/2020/4/ontology-place.owl#is_weighed_in -->

    <owl:ObjectProperty rdf:about="http://www.semanticweb.org/patriciapoveda/ontologies/2020/4/ontology-place.owl#is_weighed_in">
        <owl:inverseOf rdf:resource="http://www.semanticweb.org/patriciapoveda/ontologies/2020/4/ontology-place.owl#weighs"/>
        <rdfs:domain rdf:resource="https://apiict01.etsii.upm.es/mediawiki/index.php/User:PatriciaPoveda/ontologia.owl#Product"/>
        <rdfs:range rdf:resource="http://www.semanticweb.org/patriciapoveda/ontologies/2020/4/ontology-place.owl#Scale"/>
    </owl:ObjectProperty>
    


    <!-- http://www.semanticweb.org/patriciapoveda/ontologies/2020/4/ontology-place.owl#is_working_shcedule_of -->

    <owl:ObjectProperty rdf:about="http://www.semanticweb.org/patriciapoveda/ontologies/2020/4/ontology-place.owl#is_working_shcedule_of">
        <rdfs:domain rdf:resource="http://www.ontologydesignpatterns.org/cp/owl/timeinterval.owl#TimeInterval"/>
        <rdfs:range rdf:resource="http://www.semanticweb.org/patriciapoveda/ontologies/2020/4/ontology-place.owl#Supplier"/>
    </owl:ObjectProperty>
    


    <!-- http://www.semanticweb.org/patriciapoveda/ontologies/2020/4/ontology-place.owl#is_workplace_of -->

    <owl:ObjectProperty rdf:about="http://www.semanticweb.org/patriciapoveda/ontologies/2020/4/ontology-place.owl#is_workplace_of">
        <owl:inverseOf rdf:resource="http://www.semanticweb.org/patriciapoveda/ontologies/2020/4/ontology-place.owl#work_in"/>
        <rdfs:domain rdf:resource="http://www.semanticweb.org/patriciapoveda/ontologies/2020/4/ontology-place.owl#Load_Area"/>
        <rdfs:domain rdf:resource="http://www.semanticweb.org/patriciapoveda/ontologies/2020/4/ontology-place.owl#Sup.Manager"/>
        <rdfs:domain rdf:resource="http://www.semanticweb.org/patriciapoveda/ontologies/2020/4/ontology-place.owl#Weighing_Area"/>
        <rdfs:domain rdf:resource="https://apiict01.etsii.upm.es/mediawiki/index.php/User:PatriciaPoveda/ontologia.owl#Download_Area"/>
        <rdfs:domain rdf:resource="https://apiict01.etsii.upm.es/mediawiki/index.php/User:PatriciaPoveda/ontologia.owl#Storage_Area"/>
        <rdfs:range rdf:resource="http://www.semanticweb.org/patriciapoveda/ontologies/2020/4/ontology-place.owl#Cust.Manager"/>
        <rdfs:range rdf:resource="http://www.semanticweb.org/patriciapoveda/ontologies/2020/4/ontology-place.owl#Cust.Weighing_Worker"/>
        <rdfs:range rdf:resource="http://www.semanticweb.org/patriciapoveda/ontologies/2020/4/ontology-place.owl#Porters"/>
        <rdfs:range rdf:resource="http://www.semanticweb.org/patriciapoveda/ontologies/2020/4/ontology-place.owl#Sup.Manager"/>
        <rdfs:range rdf:resource="http://www.semanticweb.org/patriciapoveda/ontologies/2020/4/ontology-place.owl#Sup.Weighing_Worker"/>
    </owl:ObjectProperty>
    


    <!-- http://www.semanticweb.org/patriciapoveda/ontologies/2020/4/ontology-place.owl#last -->

    <owl:ObjectProperty rdf:about="http://www.semanticweb.org/patriciapoveda/ontologies/2020/4/ontology-place.owl#last">
        <rdfs:domain rdf:resource="https://apiict01.etsii.upm.es/mediawiki/index.php/User:PatriciaPoveda/ontologia.owl#Stops_Inter-segment"/>
        <rdfs:range rdf:resource="http://www.ontologydesignpatterns.org/cp/owl/timeinterval.owl#TimeInterval"/>
    </owl:ObjectProperty>
    


    <!-- http://www.semanticweb.org/patriciapoveda/ontologies/2020/4/ontology-place.owl#weighs -->

    <owl:ObjectProperty rdf:about="http://www.semanticweb.org/patriciapoveda/ontologies/2020/4/ontology-place.owl#weighs">
        <rdfs:domain rdf:resource="http://www.semanticweb.org/patriciapoveda/ontologies/2020/4/ontology-place.owl#Scale"/>
        <rdfs:range rdf:resource="https://apiict01.etsii.upm.es/mediawiki/index.php/User:PatriciaPoveda/ontologia.owl#Product"/>
    </owl:ObjectProperty>
    


    <!-- http://www.semanticweb.org/patriciapoveda/ontologies/2020/4/ontology-place.owl#work_in -->

    <owl:ObjectProperty rdf:about="http://www.semanticweb.org/patriciapoveda/ontologies/2020/4/ontology-place.owl#work_in">
        <rdfs:domain rdf:resource="http://www.semanticweb.org/patriciapoveda/ontologies/2020/4/ontology-place.owl#Cust.Manager"/>
        <rdfs:domain rdf:resource="http://www.semanticweb.org/patriciapoveda/ontologies/2020/4/ontology-place.owl#Cust.Weighing_Worker"/>
        <rdfs:domain rdf:resource="http://www.semanticweb.org/patriciapoveda/ontologies/2020/4/ontology-place.owl#Porters"/>
        <rdfs:domain rdf:resource="http://www.semanticweb.org/patriciapoveda/ontologies/2020/4/ontology-place.owl#Sup.Manager"/>
        <rdfs:domain rdf:resource="http://www.semanticweb.org/patriciapoveda/ontologies/2020/4/ontology-place.owl#Sup.Weighing_Worker"/>
        <rdfs:range rdf:resource="http://www.semanticweb.org/patriciapoveda/ontologies/2020/4/ontology-place.owl#Load_Area"/>
        <rdfs:range rdf:resource="http://www.semanticweb.org/patriciapoveda/ontologies/2020/4/ontology-place.owl#Weighing_Area"/>
        <rdfs:range rdf:resource="https://apiict01.etsii.upm.es/mediawiki/index.php/User:PatriciaPoveda/ontologia.owl#Download_Area"/>
        <rdfs:range rdf:resource="https://apiict01.etsii.upm.es/mediawiki/index.php/User:PatriciaPoveda/ontologia.owl#Storage_Area"/>
    </owl:ObjectProperty>
    


    <!-- http://www.semanticweb.org/patriciapoveda/ontologies/2020/4/ontology-place.owl#is_order/expiration_date_of -->

    <owl:ObjectProperty rdf:about="http://www.semanticweb.org/patriciapoveda/ontologies/2020/4/ontology-place.owl#is_order/expiration_date_of">
        <rdfs:domain rdf:resource="http://www.ontologydesignpatterns.org/cp/owl/timeinterval.owl#TimeInterval"/>
        <rdfs:range rdf:resource="https://apiict01.etsii.upm.es/mediawiki/index.php/User:PatriciaPoveda/ontologia.owl#Product"/>
    </owl:ObjectProperty>
    


    <!-- https://apiict01.etsii.upm.es/mediawiki/index.php/User:PatriciaPoveda/ontologia.owl#Belongs_to -->

    <owl:ObjectProperty rdf:about="https://apiict01.etsii.upm.es/mediawiki/index.php/User:PatriciaPoveda/ontologia.owl#Belongs_to">
        <owl:inverseOf rdf:resource="https://apiict01.etsii.upm.es/mediawiki/index.php/User:PatriciaPoveda/ontologia.owl#Owns"/>
        <rdfs:domain rdf:resource="https://apiict01.etsii.upm.es/mediawiki/index.php/User:PatriciaPoveda/ontologia.owl#Product"/>
        <rdfs:range rdf:resource="https://apiict01.etsii.upm.es/mediawiki/index.php/User:PatriciaPoveda/ontologia.owl#Customer"/>
        <rdfs:label>Belongs to</rdfs:label>
    </owl:ObjectProperty>
    


    <!-- https://apiict01.etsii.upm.es/mediawiki/index.php/User:PatriciaPoveda/ontologia.owl#Is_driven_by -->

    <owl:ObjectProperty rdf:about="https://apiict01.etsii.upm.es/mediawiki/index.php/User:PatriciaPoveda/ontologia.owl#Is_driven_by">
        <owl:inverseOf rdf:resource="https://apiict01.etsii.upm.es/mediawiki/index.php/User:PatriciaPoveda/ontologia.owl#Is_driver_of"/>
        <rdfs:domain rdf:resource="https://apiict01.etsii.upm.es/mediawiki/index.php/User:PatriciaPoveda/ontologia.owl#Vehicle"/>
        <rdfs:range rdf:resource="https://apiict01.etsii.upm.es/mediawiki/index.php/User:PatriciaPoveda/ontologia.owl#Driver"/>
        <rdfs:label>is driven by</rdfs:label>
    </owl:ObjectProperty>
    


    <!-- https://apiict01.etsii.upm.es/mediawiki/index.php/User:PatriciaPoveda/ontologia.owl#Is_driver_of -->

    <owl:ObjectProperty rdf:about="https://apiict01.etsii.upm.es/mediawiki/index.php/User:PatriciaPoveda/ontologia.owl#Is_driver_of">
        <rdfs:domain rdf:resource="https://apiict01.etsii.upm.es/mediawiki/index.php/User:PatriciaPoveda/ontologia.owl#Driver"/>
        <rdfs:range rdf:resource="https://apiict01.etsii.upm.es/mediawiki/index.php/User:PatriciaPoveda/ontologia.owl#Vehicle"/>
        <rdfs:label>is driver of</rdfs:label>
    </owl:ObjectProperty>
    


    <!-- https://apiict01.etsii.upm.es/mediawiki/index.php/User:PatriciaPoveda/ontologia.owl#Is_route_of -->

    <owl:ObjectProperty rdf:about="https://apiict01.etsii.upm.es/mediawiki/index.php/User:PatriciaPoveda/ontologia.owl#Is_route_of">
        <owl:inverseOf rdf:resource="https://apiict01.etsii.upm.es/mediawiki/index.php/User:PatriciaPoveda/ontologia.owl#Its_route_is"/>
        <rdfs:domain rdf:resource="https://apiict01.etsii.upm.es/mediawiki/index.php/User:PatriciaPoveda/ontologia.owl#Trajectory"/>
        <rdfs:range rdf:resource="https://apiict01.etsii.upm.es/mediawiki/index.php/User:PatriciaPoveda/ontologia.owl#Vehicle"/>
        <rdfs:label>is route of</rdfs:label>
    </owl:ObjectProperty>
    


    <!-- https://apiict01.etsii.upm.es/mediawiki/index.php/User:PatriciaPoveda/ontologia.owl#Is_stored_by -->

    <owl:ObjectProperty rdf:about="https://apiict01.etsii.upm.es/mediawiki/index.php/User:PatriciaPoveda/ontologia.owl#Is_stored_by">
        <owl:inverseOf rdf:resource="https://apiict01.etsii.upm.es/mediawiki/index.php/User:PatriciaPoveda/ontologia.owl#Store"/>
        <rdfs:domain rdf:resource="https://apiict01.etsii.upm.es/mediawiki/index.php/User:PatriciaPoveda/ontologia.owl#Product"/>
        <rdfs:range rdf:resource="http://www.semanticweb.org/patriciapoveda/ontologies/2020/4/ontology-place.owl#Product_Warehouse"/>
        <rdfs:label>is stored by</rdfs:label>
    </owl:ObjectProperty>
    


    <!-- https://apiict01.etsii.upm.es/mediawiki/index.php/User:PatriciaPoveda/ontologia.owl#Is_transported_by -->

    <owl:ObjectProperty rdf:about="https://apiict01.etsii.upm.es/mediawiki/index.php/User:PatriciaPoveda/ontologia.owl#Is_transported_by">
        <owl:inverseOf rdf:resource="https://apiict01.etsii.upm.es/mediawiki/index.php/User:PatriciaPoveda/ontologia.owl#Transport"/>
        <rdfs:domain rdf:resource="https://apiict01.etsii.upm.es/mediawiki/index.php/User:PatriciaPoveda/ontologia.owl#Product"/>
        <rdfs:range rdf:resource="https://apiict01.etsii.upm.es/mediawiki/index.php/User:PatriciaPoveda/ontologia.owl#Vehicle"/>
        <rdfs:label>is transported by</rdfs:label>
    </owl:ObjectProperty>
    


    <!-- https://apiict01.etsii.upm.es/mediawiki/index.php/User:PatriciaPoveda/ontologia.owl#Its_route_is -->

    <owl:ObjectProperty rdf:about="https://apiict01.etsii.upm.es/mediawiki/index.php/User:PatriciaPoveda/ontologia.owl#Its_route_is">
        <rdfs:domain rdf:resource="https://apiict01.etsii.upm.es/mediawiki/index.php/User:PatriciaPoveda/ontologia.owl#Vehicle"/>
        <rdfs:range rdf:resource="https://apiict01.etsii.upm.es/mediawiki/index.php/User:PatriciaPoveda/ontologia.owl#Trajectory"/>
        <rdfs:label>its route is</rdfs:label>
    </owl:ObjectProperty>
    


    <!-- https://apiict01.etsii.upm.es/mediawiki/index.php/User:PatriciaPoveda/ontologia.owl#Owns -->

    <owl:ObjectProperty rdf:about="https://apiict01.etsii.upm.es/mediawiki/index.php/User:PatriciaPoveda/ontologia.owl#Owns">
        <rdfs:domain rdf:resource="https://apiict01.etsii.upm.es/mediawiki/index.php/User:PatriciaPoveda/ontologia.owl#Customer"/>
        <rdfs:range rdf:resource="https://apiict01.etsii.upm.es/mediawiki/index.php/User:PatriciaPoveda/ontologia.owl#Product"/>
        <rdfs:label>owns</rdfs:label>
    </owl:ObjectProperty>
    


    <!-- https://apiict01.etsii.upm.es/mediawiki/index.php/User:PatriciaPoveda/ontologia.owl#Store -->

    <owl:ObjectProperty rdf:about="https://apiict01.etsii.upm.es/mediawiki/index.php/User:PatriciaPoveda/ontologia.owl#Store">
        <rdfs:domain rdf:resource="http://www.semanticweb.org/patriciapoveda/ontologies/2020/4/ontology-place.owl#Product_Warehouse"/>
        <rdfs:range rdf:resource="https://apiict01.etsii.upm.es/mediawiki/index.php/User:PatriciaPoveda/ontologia.owl#Product"/>
        <rdfs:label>stores</rdfs:label>
    </owl:ObjectProperty>
    


    <!-- https://apiict01.etsii.upm.es/mediawiki/index.php/User:PatriciaPoveda/ontologia.owl#Transport -->

    <owl:ObjectProperty rdf:about="https://apiict01.etsii.upm.es/mediawiki/index.php/User:PatriciaPoveda/ontologia.owl#Transport">
        <rdfs:domain rdf:resource="https://apiict01.etsii.upm.es/mediawiki/index.php/User:PatriciaPoveda/ontologia.owl#Vehicle"/>
        <rdfs:range rdf:resource="https://apiict01.etsii.upm.es/mediawiki/index.php/User:PatriciaPoveda/ontologia.owl#Product"/>
        <rdfs:label>transports</rdfs:label>
    </owl:ObjectProperty>
    


    <!-- 
    ///////////////////////////////////////////////////////////////////////////////////////
    //
    // Data properties
    //
    ///////////////////////////////////////////////////////////////////////////////////////
     -->

    


    <!-- http://www.ontologydesignpatterns.org/cp/owl/timeinterval.owl#hasIntervalDate -->

    <owl:DatatypeProperty rdf:about="http://www.ontologydesignpatterns.org/cp/owl/timeinterval.owl#hasIntervalDate">
        <rdfs:domain rdf:resource="http://www.ontologydesignpatterns.org/cp/owl/timeinterval.owl#TimeInterval"/>
        <rdfs:range rdf:resource="http://www.w3.org/2001/XMLSchema#string"/>
        <rdfs:comment>A datatype property that encodes values from xsd:date (or any other date-related xsd datatype) for a TimeInterval; a same TimeInterval can have more than one date value: begin date, end date, date at which the interval holds, as well as dates expressed in different formats: xsd:gYear, xsd:dateTime, etc.</rdfs:comment>
        <rdfs:isDefinedBy rdf:resource="http://www.ontologydesignpatterns.org/cp/owl/timeinterval.owl"/>
        <rdfs:label xml:lang="en">has interval date</rdfs:label>
        <rdfs:label xml:lang="it">intervallo ha data</rdfs:label>
    </owl:DatatypeProperty>
    


    <!-- http://www.ontologydesignpatterns.org/cp/owl/timeinterval.owl#hasIntervalEndDate -->

    <owl:DatatypeProperty rdf:about="http://www.ontologydesignpatterns.org/cp/owl/timeinterval.owl#hasIntervalEndDate">
        <rdfs:subPropertyOf rdf:resource="http://www.ontologydesignpatterns.org/cp/owl/timeinterval.owl#hasIntervalDate"/>
        <rdfs:domain rdf:resource="http://www.ontologydesignpatterns.org/cp/owl/timeinterval.owl#TimeInterval"/>
        <rdfs:comment>The end date of a time interval.</rdfs:comment>
        <rdfs:isDefinedBy rdf:resource="http://www.ontologydesignpatterns.org/cp/owl/timeinterval.owl"/>
        <rdfs:label xml:lang="en">interval has end date</rdfs:label>
    </owl:DatatypeProperty>
    


    <!-- http://www.ontologydesignpatterns.org/cp/owl/timeinterval.owl#hasIntervalStartDate -->

    <owl:DatatypeProperty rdf:about="http://www.ontologydesignpatterns.org/cp/owl/timeinterval.owl#hasIntervalStartDate">
        <rdfs:subPropertyOf rdf:resource="http://www.ontologydesignpatterns.org/cp/owl/timeinterval.owl#hasIntervalDate"/>
        <rdfs:domain rdf:resource="http://www.ontologydesignpatterns.org/cp/owl/timeinterval.owl#TimeInterval"/>
        <rdfs:comment>The start date of a time interval.</rdfs:comment>
        <rdfs:isDefinedBy rdf:resource="http://www.ontologydesignpatterns.org/cp/owl/timeinterval.owl"/>
        <rdfs:label xml:lang="en">interval has start date</rdfs:label>
    </owl:DatatypeProperty>
    


    <!-- http://www.semanticweb.org/patriciapoveda/ontologies/2020/4/ontology-place.owl#End_Point -->

    <owl:DatatypeProperty rdf:about="http://www.semanticweb.org/patriciapoveda/ontologies/2020/4/ontology-place.owl#End_Point">
        <rdfs:domain rdf:resource="https://apiict01.etsii.upm.es/mediawiki/index.php/User:PatriciaPoveda/ontologia.owl#Trajectory"/>
        <rdfs:range rdf:resource="http://www.w3.org/2001/XMLSchema#string"/>
        <rdfs:comment xml:lang="en">Geographical point where the route ends, normally the vehicule garage where the vehicule was parked at the beginning.</rdfs:comment>
        <rdfs:comment xml:lang="es">Punto geográfico en el que termina la ruta, normalmente el garaje desde donde ha salido el vehiculo.
La rutas generalmente son cerradas</rdfs:comment>
    </owl:DatatypeProperty>
    


    <!-- http://www.semanticweb.org/patriciapoveda/ontologies/2020/4/ontology-place.owl#ID_Download -->

    <owl:DatatypeProperty rdf:about="http://www.semanticweb.org/patriciapoveda/ontologies/2020/4/ontology-place.owl#ID_Download">
        <rdfs:subPropertyOf rdf:resource="https://apiict01.etsii.upm.es/mediawiki/index.php/User:PatriciaPoveda/ontologia.owl#Identifier"/>
        <rdfs:domain rdf:resource="http://www.semanticweb.org/patriciapoveda/ontologies/2020/4/ontology-place.owl#Download"/>
        <rdfs:range rdf:resource="http://www.w3.org/2001/XMLSchema#string"/>
    </owl:DatatypeProperty>
    


    <!-- http://www.semanticweb.org/patriciapoveda/ontologies/2020/4/ontology-place.owl#ID_Trajectory -->

    <owl:DatatypeProperty rdf:about="http://www.semanticweb.org/patriciapoveda/ontologies/2020/4/ontology-place.owl#ID_Trajectory">
        <rdfs:subPropertyOf rdf:resource="https://apiict01.etsii.upm.es/mediawiki/index.php/User:PatriciaPoveda/ontologia.owl#Identifier"/>
        <rdfs:domain rdf:resource="https://apiict01.etsii.upm.es/mediawiki/index.php/User:PatriciaPoveda/ontologia.owl#Trajectory"/>
        <rdfs:range rdf:resource="http://www.w3.org/2001/XMLSchema#string"/>
    </owl:DatatypeProperty>
    


    <!-- http://www.semanticweb.org/patriciapoveda/ontologies/2020/4/ontology-place.owl#Nature_of_material -->

    <owl:DatatypeProperty rdf:about="http://www.semanticweb.org/patriciapoveda/ontologies/2020/4/ontology-place.owl#Nature_of_material">
        <rdfs:domain rdf:resource="https://apiict01.etsii.upm.es/mediawiki/index.php/User:PatriciaPoveda/ontologia.owl#Product"/>
        <rdfs:range rdf:resource="http://www.w3.org/2001/XMLSchema#string"/>
        <rdfs:comment xml:lang="es">Naturaleza del material. Para diferenciar entre tipos de metales.</rdfs:comment>
        <rdfs:comment xml:lang="en">Nature of the material. To classify between different types of metals.</rdfs:comment>
    </owl:DatatypeProperty>
    


    <!-- http://www.semanticweb.org/patriciapoveda/ontologies/2020/4/ontology-place.owl#Occupation_Level -->

    <owl:DatatypeProperty rdf:about="http://www.semanticweb.org/patriciapoveda/ontologies/2020/4/ontology-place.owl#Occupation_Level">
        <rdfs:domain rdf:resource="http://www.semanticweb.org/patriciapoveda/ontologies/2020/4/ontology-place.owl#Areas"/>
        <rdfs:range rdf:resource="http://www.w3.org/2001/XMLSchema#string"/>
    </owl:DatatypeProperty>
    


    <!-- http://www.semanticweb.org/patriciapoveda/ontologies/2020/4/ontology-place.owl#Quality_Level_of_Material -->

    <owl:DatatypeProperty rdf:about="http://www.semanticweb.org/patriciapoveda/ontologies/2020/4/ontology-place.owl#Quality_Level_of_Material">
        <rdfs:domain rdf:resource="https://apiict01.etsii.upm.es/mediawiki/index.php/User:PatriciaPoveda/ontologia.owl#Product"/>
        <rdfs:range rdf:resource="http://www.w3.org/2001/XMLSchema#string"/>
        <rdfs:comment xml:lang="es">Calidad del material segun la cual los materiales tendrán un valor u otro.</rdfs:comment>
        <rdfs:comment xml:lang="en">Quality of the material, according to it, the materials will have more or less value.</rdfs:comment>
    </owl:DatatypeProperty>
    


    <!-- http://www.semanticweb.org/patriciapoveda/ontologies/2020/4/ontology-place.owl#Start_Point -->

    <owl:DatatypeProperty rdf:about="http://www.semanticweb.org/patriciapoveda/ontologies/2020/4/ontology-place.owl#Start_Point">
        <rdfs:domain rdf:resource="https://apiict01.etsii.upm.es/mediawiki/index.php/User:PatriciaPoveda/ontologia.owl#Trajectory"/>
        <rdfs:range rdf:resource="http://www.w3.org/2001/XMLSchema#string"/>
        <rdfs:comment xml:lang="en">Geographical point where the route begins, generally the vehicle garage.</rdfs:comment>
        <rdfs:comment xml:lang="es">Punto geográfico en el que comienza una ruta, desde donde salen los camiones (los garajes)</rdfs:comment>
    </owl:DatatypeProperty>
    


    <!-- https://apiict01.etsii.upm.es/mediawiki/index.php/User:PatriciaPoveda/ontologia.owl#Adress_Customer -->

    <owl:DatatypeProperty rdf:about="https://apiict01.etsii.upm.es/mediawiki/index.php/User:PatriciaPoveda/ontologia.owl#Adress_Customer">
        <rdfs:subPropertyOf rdf:resource="https://apiict01.etsii.upm.es/mediawiki/index.php/User:PatriciaPoveda/ontologia.owl#Location"/>
        <rdfs:domain rdf:resource="https://apiict01.etsii.upm.es/mediawiki/index.php/User:PatriciaPoveda/ontologia.owl#Customer"/>
        <rdfs:range rdf:resource="http://www.w3.org/2001/XMLSchema#string"/>
    </owl:DatatypeProperty>
    


    <!-- https://apiict01.etsii.upm.es/mediawiki/index.php/User:PatriciaPoveda/ontologia.owl#Adress_Warehouse -->

    <owl:DatatypeProperty rdf:about="https://apiict01.etsii.upm.es/mediawiki/index.php/User:PatriciaPoveda/ontologia.owl#Adress_Warehouse">
        <rdfs:subPropertyOf rdf:resource="https://apiict01.etsii.upm.es/mediawiki/index.php/User:PatriciaPoveda/ontologia.owl#Location"/>
        <rdfs:domain rdf:resource="https://apiict01.etsii.upm.es/mediawiki/index.php/User:PatriciaPoveda/ontologia.owl#Warehouses"/>
        <rdfs:range rdf:resource="http://www.w3.org/2001/XMLSchema#string"/>
    </owl:DatatypeProperty>
    


    <!-- https://apiict01.etsii.upm.es/mediawiki/index.php/User:PatriciaPoveda/ontologia.owl#Capac_Vehicle -->

    <owl:DatatypeProperty rdf:about="https://apiict01.etsii.upm.es/mediawiki/index.php/User:PatriciaPoveda/ontologia.owl#Capac_Vehicle">
        <rdfs:subPropertyOf rdf:resource="https://apiict01.etsii.upm.es/mediawiki/index.php/User:PatriciaPoveda/ontologia.owl#Capacity"/>
        <rdfs:domain rdf:resource="https://apiict01.etsii.upm.es/mediawiki/index.php/User:PatriciaPoveda/ontologia.owl#Vehicle"/>
        <rdfs:range rdf:resource="http://www.w3.org/2001/XMLSchema#float"/>
    </owl:DatatypeProperty>
    


    <!-- https://apiict01.etsii.upm.es/mediawiki/index.php/User:PatriciaPoveda/ontologia.owl#Capac_Warehouse -->

    <owl:DatatypeProperty rdf:about="https://apiict01.etsii.upm.es/mediawiki/index.php/User:PatriciaPoveda/ontologia.owl#Capac_Warehouse">
        <rdfs:subPropertyOf rdf:resource="https://apiict01.etsii.upm.es/mediawiki/index.php/User:PatriciaPoveda/ontologia.owl#Capacity"/>
        <rdfs:domain rdf:resource="https://apiict01.etsii.upm.es/mediawiki/index.php/User:PatriciaPoveda/ontologia.owl#Warehouses"/>
        <rdfs:range rdf:resource="http://www.w3.org/2001/XMLSchema#float"/>
    </owl:DatatypeProperty>
    


    <!-- https://apiict01.etsii.upm.es/mediawiki/index.php/User:PatriciaPoveda/ontologia.owl#Capacity -->

    <owl:DatatypeProperty rdf:about="https://apiict01.etsii.upm.es/mediawiki/index.php/User:PatriciaPoveda/ontologia.owl#Capacity">
        <rdfs:range rdf:resource="http://www.w3.org/2001/XMLSchema#float"/>
        <rdfs:comment xml:lang="en">It registers the capacity of different elements, such as vehicles, warehouses, or the occupation level of warehouse scales, to see if they can continue taking over more material or they are fulfilled.</rdfs:comment>
        <rdfs:comment xml:lang="es">Recoge la capacidad de los distintos elementos, como los vehiculos, almacenes, o la ocupación de básculas de los almacenes, para saber si pueden seguir haciendose cargo de más material.</rdfs:comment>
    </owl:DatatypeProperty>
    


    <!-- https://apiict01.etsii.upm.es/mediawiki/index.php/User:PatriciaPoveda/ontologia.owl#Dimension -->

    <owl:DatatypeProperty rdf:about="https://apiict01.etsii.upm.es/mediawiki/index.php/User:PatriciaPoveda/ontologia.owl#Dimension">
        <rdfs:subPropertyOf rdf:resource="https://apiict01.etsii.upm.es/mediawiki/index.php/User:PatriciaPoveda/ontologia.owl#Parameters"/>
        <rdfs:domain rdf:resource="https://apiict01.etsii.upm.es/mediawiki/index.php/User:PatriciaPoveda/ontologia.owl#Product"/>
        <rdfs:domain rdf:resource="https://apiict01.etsii.upm.es/mediawiki/index.php/User:PatriciaPoveda/ontologia.owl#Vehicle"/>
        <rdfs:range rdf:resource="http://www.w3.org/2001/XMLSchema#string"/>
    </owl:DatatypeProperty>
    


    <!-- https://apiict01.etsii.upm.es/mediawiki/index.php/User:PatriciaPoveda/ontologia.owl#Experience -->

    <owl:DatatypeProperty rdf:about="https://apiict01.etsii.upm.es/mediawiki/index.php/User:PatriciaPoveda/ontologia.owl#Experience">
        <rdfs:domain rdf:resource="http://www.semanticweb.org/patriciapoveda/ontologies/2020/4/ontology-place.owl#Supplier"/>
        <rdfs:range rdf:resource="http://www.w3.org/2001/XMLSchema#string"/>
        <rdfs:comment xml:lang="en">It represents the experience level of the people involved on the process. The assignment of the tasks and routes will depend on it</rdfs:comment>
        <rdfs:comment xml:lang="es">Recoge el nivel de experiencia de las personas que particpan en el proceso. De ello dependerá la asignación de unos encargos u otros</rdfs:comment>
    </owl:DatatypeProperty>
    


    <!-- https://apiict01.etsii.upm.es/mediawiki/index.php/User:PatriciaPoveda/ontologia.owl#Fuel -->

    <owl:DatatypeProperty rdf:about="https://apiict01.etsii.upm.es/mediawiki/index.php/User:PatriciaPoveda/ontologia.owl#Fuel">
        <rdfs:domain rdf:resource="https://apiict01.etsii.upm.es/mediawiki/index.php/User:PatriciaPoveda/ontologia.owl#Vehicle"/>
        <rdfs:range rdf:resource="http://www.w3.org/2001/XMLSchema#float"/>
        <rdfs:comment xml:lang="en">It collects the fuel level of the vehicles, in order to know if it is necessary for the trucks to get out of the route and refuel.</rdfs:comment>
        <rdfs:comment xml:lang="es">Recoge el nivel de combustible de los vehiculos para saber si es necesario que se desvien a repostar.</rdfs:comment>
    </owl:DatatypeProperty>
    


    <!-- https://apiict01.etsii.upm.es/mediawiki/index.php/User:PatriciaPoveda/ontologia.owl#ID_Customer -->

    <owl:DatatypeProperty rdf:about="https://apiict01.etsii.upm.es/mediawiki/index.php/User:PatriciaPoveda/ontologia.owl#ID_Customer">
        <rdfs:subPropertyOf rdf:resource="https://apiict01.etsii.upm.es/mediawiki/index.php/User:PatriciaPoveda/ontologia.owl#Identifier"/>
        <rdfs:domain rdf:resource="https://apiict01.etsii.upm.es/mediawiki/index.php/User:PatriciaPoveda/ontologia.owl#Customer"/>
        <rdfs:range rdf:resource="http://www.w3.org/2001/XMLSchema#string"/>
    </owl:DatatypeProperty>
    


    <!-- https://apiict01.etsii.upm.es/mediawiki/index.php/User:PatriciaPoveda/ontologia.owl#ID_Product -->

    <owl:DatatypeProperty rdf:about="https://apiict01.etsii.upm.es/mediawiki/index.php/User:PatriciaPoveda/ontologia.owl#ID_Product">
        <rdfs:subPropertyOf rdf:resource="https://apiict01.etsii.upm.es/mediawiki/index.php/User:PatriciaPoveda/ontologia.owl#Identifier"/>
        <rdfs:domain rdf:resource="https://apiict01.etsii.upm.es/mediawiki/index.php/User:PatriciaPoveda/ontologia.owl#Product"/>
        <rdfs:range rdf:resource="http://www.w3.org/2001/XMLSchema#string"/>
    </owl:DatatypeProperty>
    


    <!-- https://apiict01.etsii.upm.es/mediawiki/index.php/User:PatriciaPoveda/ontologia.owl#ID_Supplier -->

    <owl:DatatypeProperty rdf:about="https://apiict01.etsii.upm.es/mediawiki/index.php/User:PatriciaPoveda/ontologia.owl#ID_Supplier">
        <rdfs:subPropertyOf rdf:resource="https://apiict01.etsii.upm.es/mediawiki/index.php/User:PatriciaPoveda/ontologia.owl#Identifier"/>
        <rdfs:domain rdf:resource="http://www.semanticweb.org/patriciapoveda/ontologies/2020/4/ontology-place.owl#Supplier"/>
        <rdfs:range rdf:resource="http://www.w3.org/2001/XMLSchema#string"/>
    </owl:DatatypeProperty>
    


    <!-- https://apiict01.etsii.upm.es/mediawiki/index.php/User:PatriciaPoveda/ontologia.owl#ID_Vehicle -->

    <owl:DatatypeProperty rdf:about="https://apiict01.etsii.upm.es/mediawiki/index.php/User:PatriciaPoveda/ontologia.owl#ID_Vehicle">
        <rdfs:subPropertyOf rdf:resource="https://apiict01.etsii.upm.es/mediawiki/index.php/User:PatriciaPoveda/ontologia.owl#Identifier"/>
        <rdfs:domain rdf:resource="https://apiict01.etsii.upm.es/mediawiki/index.php/User:PatriciaPoveda/ontologia.owl#Vehicle"/>
        <rdfs:range rdf:resource="http://www.w3.org/2001/XMLSchema#string"/>
    </owl:DatatypeProperty>
    


    <!-- https://apiict01.etsii.upm.es/mediawiki/index.php/User:PatriciaPoveda/ontologia.owl#Identifier -->

    <owl:DatatypeProperty rdf:about="https://apiict01.etsii.upm.es/mediawiki/index.php/User:PatriciaPoveda/ontologia.owl#Identifier">
        <rdfs:range rdf:resource="http://www.w3.org/2001/XMLSchema#string"/>
        <rdfs:comment xml:lang="en">An identification number is assigned to the different elements to be able to identify them and keep track of them in a simple way: it is applied to customers, drivers, vehicles and products.</rdfs:comment>
        <rdfs:comment xml:lang="es">Se adjudica un numero de identificación a los distintos elementos para poder identificarlos y llevar un seguimiento de ellos de forma sencilla: se aplica a los clientes, conductores, vehiculos y productos.</rdfs:comment>
    </owl:DatatypeProperty>
    


    <!-- https://apiict01.etsii.upm.es/mediawiki/index.php/User:PatriciaPoveda/ontologia.owl#Load -->

    <owl:DatatypeProperty rdf:about="https://apiict01.etsii.upm.es/mediawiki/index.php/User:PatriciaPoveda/ontologia.owl#Load">
        <rdfs:subPropertyOf rdf:resource="https://apiict01.etsii.upm.es/mediawiki/index.php/User:PatriciaPoveda/ontologia.owl#Parameters"/>
        <rdfs:domain rdf:resource="https://apiict01.etsii.upm.es/mediawiki/index.php/User:PatriciaPoveda/ontologia.owl#Product"/>
        <rdfs:domain rdf:resource="https://apiict01.etsii.upm.es/mediawiki/index.php/User:PatriciaPoveda/ontologia.owl#Vehicle"/>
        <rdfs:range rdf:resource="http://www.w3.org/2001/XMLSchema#string"/>
    </owl:DatatypeProperty>
    


    <!-- https://apiict01.etsii.upm.es/mediawiki/index.php/User:PatriciaPoveda/ontologia.owl#Location -->

    <owl:DatatypeProperty rdf:about="https://apiict01.etsii.upm.es/mediawiki/index.php/User:PatriciaPoveda/ontologia.owl#Location">
        <rdfs:range rdf:resource="http://www.w3.org/2001/XMLSchema#string"/>
        <rdfs:comment xml:lang="en">It represents the addresses of the customers pick up points, of the departure and arrival warehouses, and the real-time positions of the vehicles and drivers in order to achieve an optimal service.
The model is limited to a regional area with not too big distances (radius of 100 km approx)</rdfs:comment>
        <rdfs:comment xml:lang="es">Recoge las direcciones de los puntos de recogida de los clientes, de los almacenes de partida y llegada, y las posiciones en tiempo real de los vehiculos y conductores para un servicio optimo.
El modelo se limita a una zona regional con distancias no demasiado grandes (radio de 100 km aprox)</rdfs:comment>
    </owl:DatatypeProperty>
    


    <!-- https://apiict01.etsii.upm.es/mediawiki/index.php/User:PatriciaPoveda/ontologia.owl#Name -->

    <owl:DatatypeProperty rdf:about="https://apiict01.etsii.upm.es/mediawiki/index.php/User:PatriciaPoveda/ontologia.owl#Name">
        <rdfs:domain rdf:resource="http://www.semanticweb.org/patriciapoveda/ontologies/2020/4/ontology-place.owl#Supplier"/>
        <rdfs:domain rdf:resource="https://apiict01.etsii.upm.es/mediawiki/index.php/User:PatriciaPoveda/ontologia.owl#Customer"/>
        <rdfs:range rdf:resource="http://www.w3.org/2001/XMLSchema#string"/>
        <rdfs:comment xml:lang="es">Se registra el nombre de los clientes y proveedores para poder idetificarlos</rdfs:comment>
        <rdfs:comment xml:lang="en">The names of customers and suppliers are registered in order to identify them properly</rdfs:comment>
    </owl:DatatypeProperty>
    


    <!-- https://apiict01.etsii.upm.es/mediawiki/index.php/User:PatriciaPoveda/ontologia.owl#Parameters -->

    <owl:DatatypeProperty rdf:about="https://apiict01.etsii.upm.es/mediawiki/index.php/User:PatriciaPoveda/ontologia.owl#Parameters">
        <rdfs:comment xml:lang="en">Dimensions and weights of vehicles or products</rdfs:comment>
        <rdfs:comment xml:lang="es">Medidas y peso, de los vehiculos o los productos</rdfs:comment>
    </owl:DatatypeProperty>
    


    <!-- https://apiict01.etsii.upm.es/mediawiki/index.php/User:PatriciaPoveda/ontologia.owl#Path_Length -->

    <owl:DatatypeProperty rdf:about="https://apiict01.etsii.upm.es/mediawiki/index.php/User:PatriciaPoveda/ontologia.owl#Path_Length">
        <rdfs:domain rdf:resource="https://apiict01.etsii.upm.es/mediawiki/index.php/User:PatriciaPoveda/ontologia.owl#Trajectory"/>
        <rdfs:range rdf:resource="http://www.w3.org/2001/XMLSchema#string"/>
        <rdfs:comment xml:lang="en">Sum of all the segments that make up a route: it has a direct influence in the duration of the route</rdfs:comment>
        <rdfs:comment xml:lang="es">Total de los segmentos que componen una ruta: influyen en el tiempo de duracion de una ruta</rdfs:comment>
    </owl:DatatypeProperty>
    


    <!-- https://apiict01.etsii.upm.es/mediawiki/index.php/User:PatriciaPoveda/ontologia.owl#Path_Stops -->

    <owl:DatatypeProperty rdf:about="https://apiict01.etsii.upm.es/mediawiki/index.php/User:PatriciaPoveda/ontologia.owl#Path_Stops">
        <rdfs:domain rdf:resource="https://apiict01.etsii.upm.es/mediawiki/index.php/User:PatriciaPoveda/ontologia.owl#Trajectory"/>
        <rdfs:range rdf:resource="http://www.w3.org/2001/XMLSchema#integer"/>
        <rdfs:comment xml:lang="en">Number of stops that componed a route. They have a direct effect on the duration of the route</rdfs:comment>
        <rdfs:comment xml:lang="es">Número de paradas que componen la ruta. Tendrán un efecto directo en la duración de la ruta</rdfs:comment>
    </owl:DatatypeProperty>
    


    <!-- https://apiict01.etsii.upm.es/mediawiki/index.php/User:PatriciaPoveda/ontologia.owl#State -->

    <owl:DatatypeProperty rdf:about="https://apiict01.etsii.upm.es/mediawiki/index.php/User:PatriciaPoveda/ontologia.owl#State">
        <rdfs:domain rdf:resource="http://www.semanticweb.org/patriciapoveda/ontologies/2020/4/ontology-place.owl#Supplier"/>
        <rdfs:domain rdf:resource="https://apiict01.etsii.upm.es/mediawiki/index.php/User:PatriciaPoveda/ontologia.owl#Download_Area"/>
        <rdfs:domain rdf:resource="https://apiict01.etsii.upm.es/mediawiki/index.php/User:PatriciaPoveda/ontologia.owl#Storage_Area"/>
        <rdfs:domain rdf:resource="https://apiict01.etsii.upm.es/mediawiki/index.php/User:PatriciaPoveda/ontologia.owl#Vehicle"/>
        <rdfs:range rdf:resource="http://www.w3.org/2001/XMLSchema#string"/>
        <rdfs:comment xml:lang="es">Determina la situacion del objeto: Libre/Ocupado
Se aplica a los conductores y a los vehiculos para saber si se les puede destinar a nueva ruta, y a las zonas de los almacenes para saber si el vehiculo puede entrar</rdfs:comment>
        <rdfs:comment xml:lang="en">It determines the state of the object: Free / Busy
It is applied to drivers and vehicles, in order to know if they can be assigned to a new route, and to warehouse areas to know if another vehicle can enter</rdfs:comment>
    </owl:DatatypeProperty>
    


    <!-- https://apiict01.etsii.upm.es/mediawiki/index.php/User:PatriciaPoveda/ontologia.owl#Traffic -->

    <owl:DatatypeProperty rdf:about="https://apiict01.etsii.upm.es/mediawiki/index.php/User:PatriciaPoveda/ontologia.owl#Traffic">
        <rdfs:domain rdf:resource="https://apiict01.etsii.upm.es/mediawiki/index.php/User:PatriciaPoveda/ontologia.owl#Trajectory"/>
        <rdfs:range rdf:resource="http://www.w3.org/2001/XMLSchema#string"/>
        <rdfs:comment xml:lang="es">Ayuda a determinar cuales son las rutas más apropiadas y desviarlas si hiciese falta</rdfs:comment>
        <rdfs:comment xml:lang="en">It helps to determine which are the most appropriate routes for the tasks and to divert them if necessary</rdfs:comment>
    </owl:DatatypeProperty>
    


    <!-- https://apiict01.etsii.upm.es/mediawiki/index.php/User:PatriciaPoveda/ontologia.owl#Urgency -->

    <owl:DatatypeProperty rdf:about="https://apiict01.etsii.upm.es/mediawiki/index.php/User:PatriciaPoveda/ontologia.owl#Urgency">
        <rdfs:domain rdf:resource="http://www.semanticweb.org/patriciapoveda/ontologies/2020/4/ontology-place.owl#Scheduling"/>
        <rdfs:range rdf:resource="http://www.w3.org/2001/XMLSchema#string"/>
        <rdfs:comment xml:lang="es">Determinan la prioridad y el orden de los encargos</rdfs:comment>
        <rdfs:comment xml:lang="en">Determine the priority of orders</rdfs:comment>
    </owl:DatatypeProperty>
    


    <!-- 
    ///////////////////////////////////////////////////////////////////////////////////////
    //
    // Classes
    //
    ///////////////////////////////////////////////////////////////////////////////////////
     -->

    


    <!-- http://www.ontologydesignpatterns.org/cp/owl/place.owl#Place -->

    <owl:Class rdf:about="http://www.ontologydesignpatterns.org/cp/owl/place.owl#Place">
        <owl:equivalentClass>
            <owl:Restriction>
                <owl:onProperty rdf:resource="http://www.ontologydesignpatterns.org/cp/owl/place.owl#isLocationOf"/>
                <owl:someValuesFrom rdf:resource="http://www.w3.org/2002/07/owl#Thing"/>
            </owl:Restriction>
        </owl:equivalentClass>
        <rdfs:comment>A location, in a very generic sense: a political geographic entity (Roma, Lesotho), a location determined by the presence of other entities (&apos;the area close to Roma&apos;), pivot events or signs (&quot;the area where the helicopter fell&quot;), complements of other entities (&apos;the area under the table&apos;), as well as physical objects conceptualized as locations as their main identity criterion (&apos;the territory of Italy&apos;).
In this generic sense, a Place is an &apos;approximate&apos;, relative location. For an &apos;absolute&apos;, abstract location, cf. the pattern spaceregion.owl.
Formally, a Place is defined by the fact of having something located in it; a Place is located in itself.</rdfs:comment>
        <rdfs:isDefinedBy rdf:resource="http://www.ontologydesignpatterns.org/cp/owl/place.owl"/>
        <rdfs:label xml:lang="en">Place</rdfs:label>
    </owl:Class>
    


    <!-- http://www.ontologydesignpatterns.org/cp/owl/timeinterval.owl#TimeInterval -->

    <owl:Class rdf:about="http://www.ontologydesignpatterns.org/cp/owl/timeinterval.owl#TimeInterval">
        <rdfs:subClassOf>
            <owl:Restriction>
                <owl:onProperty rdf:resource="http://www.ontologydesignpatterns.org/cp/owl/timeinterval.owl#hasIntervalEndDate"/>
                <owl:maxCardinality rdf:datatype="http://www.w3.org/2001/XMLSchema#nonNegativeInteger">1</owl:maxCardinality>
            </owl:Restriction>
        </rdfs:subClassOf>
        <rdfs:subClassOf>
            <owl:Restriction>
                <owl:onProperty rdf:resource="http://www.ontologydesignpatterns.org/cp/owl/timeinterval.owl#hasIntervalStartDate"/>
                <owl:maxCardinality rdf:datatype="http://www.w3.org/2001/XMLSchema#nonNegativeInteger">1</owl:maxCardinality>
            </owl:Restriction>
        </rdfs:subClassOf>
        <rdfs:comment>Any Region in a dimensional space that aims at representing time.
It should be used when you want to talk about time as an object having some characteristics.</rdfs:comment>
        <rdfs:isDefinedBy rdf:resource="http://www.ontologydesignpatterns.org/cp/owl/timeinterval.owl"/>
        <rdfs:label xml:lang="en">Time interval</rdfs:label>
    </owl:Class>
    


    <!-- http://www.semanticweb.org/patriciapoveda/ontologies/2020/4/ontology-place.owl#Activities -->

    <owl:Class rdf:about="http://www.semanticweb.org/patriciapoveda/ontologies/2020/4/ontology-place.owl#Activities">
        <rdfs:subClassOf rdf:resource="http://www.semanticweb.org/patriciapoveda/ontologies/2020/4/ontology-place.owl#Logistics_Services"/>
        <rdfs:comment xml:lang="es">Distintas acciones relevantes en el proceso de logística. Se distinguirán subclases según las distintas actividades. Estas actividades se pueden utilizar para componer actividades más complejas.</rdfs:comment>
        <rdfs:comment xml:lang="en">Relevant actions in the logistics process. Subclasses will be distinguished according to the different activities. These activities can be used to compose more complex activities.</rdfs:comment>
    </owl:Class>
    


    <!-- http://www.semanticweb.org/patriciapoveda/ontologies/2020/4/ontology-place.owl#Areas -->

    <owl:Class rdf:about="http://www.semanticweb.org/patriciapoveda/ontologies/2020/4/ontology-place.owl#Areas">
        <rdfs:subClassOf rdf:resource="http://www.semanticweb.org/patriciapoveda/ontologies/2020/4/ontology-place.owl#Logistics_Resources"/>
        <rdfs:comment xml:lang="es">Dentro de los almacenes y locales de los clientes es necesario distinguir entre distintas zonas según la actividad que se realiza en ellos</rdfs:comment>
        <rdfs:comment xml:lang="en">Within customers&apos; warehouses and premises, it is necessary to make a difference between the areas according to the activity carried out in them.</rdfs:comment>
    </owl:Class>
    


    <!-- http://www.semanticweb.org/patriciapoveda/ontologies/2020/4/ontology-place.owl#Box_Crane -->

    <owl:Class rdf:about="http://www.semanticweb.org/patriciapoveda/ontologies/2020/4/ontology-place.owl#Box_Crane">
        <owl:equivalentClass rdf:resource="http://www.semanticweb.org/patriciapoveda/ontologies/2020/4/ontology-place.owl#Box_with_Crane"/>
        <rdfs:subClassOf rdf:resource="https://apiict01.etsii.upm.es/mediawiki/index.php/User:PatriciaPoveda/ontologia.owl#Truck_Crane"/>
    </owl:Class>
    


    <!-- http://www.semanticweb.org/patriciapoveda/ontologies/2020/4/ontology-place.owl#Box_with_Crane -->

    <owl:Class rdf:about="http://www.semanticweb.org/patriciapoveda/ontologies/2020/4/ontology-place.owl#Box_with_Crane">
        <rdfs:subClassOf rdf:resource="https://apiict01.etsii.upm.es/mediawiki/index.php/User:PatriciaPoveda/ontologia.owl#Truck_Box"/>
        <owl:disjointWith rdf:resource="http://www.semanticweb.org/patriciapoveda/ontologies/2020/4/ontology-place.owl#Box_without_Crane"/>
    </owl:Class>
    


    <!-- http://www.semanticweb.org/patriciapoveda/ontologies/2020/4/ontology-place.owl#Box_without_Crane -->

    <owl:Class rdf:about="http://www.semanticweb.org/patriciapoveda/ontologies/2020/4/ontology-place.owl#Box_without_Crane">
        <rdfs:subClassOf rdf:resource="https://apiict01.etsii.upm.es/mediawiki/index.php/User:PatriciaPoveda/ontologia.owl#Truck_Box"/>
    </owl:Class>
    


    <!-- http://www.semanticweb.org/patriciapoveda/ontologies/2020/4/ontology-place.owl#Break_Stop -->

    <owl:Class rdf:about="http://www.semanticweb.org/patriciapoveda/ontologies/2020/4/ontology-place.owl#Break_Stop">
        <rdfs:subClassOf rdf:resource="https://apiict01.etsii.upm.es/mediawiki/index.php/User:PatriciaPoveda/ontologia.owl#Stops_Inter-segment"/>
    </owl:Class>
    


    <!-- http://www.semanticweb.org/patriciapoveda/ontologies/2020/4/ontology-place.owl#Cust.Manager -->

    <owl:Class rdf:about="http://www.semanticweb.org/patriciapoveda/ontologies/2020/4/ontology-place.owl#Cust.Manager">
        <rdfs:subClassOf rdf:resource="https://apiict01.etsii.upm.es/mediawiki/index.php/User:PatriciaPoveda/ontologia.owl#Customer"/>
        <rdfs:comment xml:lang="en">People in charge of leading the process from the customer&apos; position, leading the customers team and making decisions</rdfs:comment>
        <rdfs:comment xml:lang="es">Personas encargadas de dirigir el proceso referente a la parte del cliente, dirigiendo a los basculistas e indicando a los proveedores.</rdfs:comment>
    </owl:Class>
    


    <!-- http://www.semanticweb.org/patriciapoveda/ontologies/2020/4/ontology-place.owl#Cust.Weighing_Worker -->

    <owl:Class rdf:about="http://www.semanticweb.org/patriciapoveda/ontologies/2020/4/ontology-place.owl#Cust.Weighing_Worker">
        <rdfs:subClassOf rdf:resource="https://apiict01.etsii.upm.es/mediawiki/index.php/User:PatriciaPoveda/ontologia.owl#Customer"/>
        <rdfs:comment xml:lang="en">People that are in charge of weighing the product when the truck is going to pick it up in the customer premises, weighing the truck when entering and leaving the place to calculate the load difference.</rdfs:comment>
        <rdfs:comment xml:lang="es">Personas encargadas de pesar el producto cuando el camión lo recoge, pesando el camión al entrar y al salir para calcular la diferencia de carga.</rdfs:comment>
    </owl:Class>
    


    <!-- http://www.semanticweb.org/patriciapoveda/ontologies/2020/4/ontology-place.owl#Cust_Scale_Entry -->

    <owl:Class rdf:about="http://www.semanticweb.org/patriciapoveda/ontologies/2020/4/ontology-place.owl#Cust_Scale_Entry">
        <rdfs:subClassOf rdf:resource="http://www.semanticweb.org/patriciapoveda/ontologies/2020/4/ontology-place.owl#Customer_Scale"/>
    </owl:Class>
    


    <!-- http://www.semanticweb.org/patriciapoveda/ontologies/2020/4/ontology-place.owl#Cust_Scale_Exit -->

    <owl:Class rdf:about="http://www.semanticweb.org/patriciapoveda/ontologies/2020/4/ontology-place.owl#Cust_Scale_Exit">
        <rdfs:subClassOf rdf:resource="http://www.semanticweb.org/patriciapoveda/ontologies/2020/4/ontology-place.owl#Customer_Scale"/>
    </owl:Class>
    


    <!-- http://www.semanticweb.org/patriciapoveda/ontologies/2020/4/ontology-place.owl#Customer_Scale -->

    <owl:Class rdf:about="http://www.semanticweb.org/patriciapoveda/ontologies/2020/4/ontology-place.owl#Customer_Scale">
        <rdfs:subClassOf rdf:resource="http://www.semanticweb.org/patriciapoveda/ontologies/2020/4/ontology-place.owl#Scale"/>
    </owl:Class>
    


    <!-- http://www.semanticweb.org/patriciapoveda/ontologies/2020/4/ontology-place.owl#Customer_Storage_Area -->

    <owl:Class rdf:about="http://www.semanticweb.org/patriciapoveda/ontologies/2020/4/ontology-place.owl#Customer_Storage_Area">
        <rdfs:subClassOf rdf:resource="https://apiict01.etsii.upm.es/mediawiki/index.php/User:PatriciaPoveda/ontologia.owl#Storage_Area"/>
        <owl:disjointWith rdf:resource="http://www.semanticweb.org/patriciapoveda/ontologies/2020/4/ontology-place.owl#Warehouse_Storage_Area"/>
    </owl:Class>
    


    <!-- http://www.semanticweb.org/patriciapoveda/ontologies/2020/4/ontology-place.owl#Customer_Weighing_Area -->

    <owl:Class rdf:about="http://www.semanticweb.org/patriciapoveda/ontologies/2020/4/ontology-place.owl#Customer_Weighing_Area">
        <rdfs:subClassOf rdf:resource="http://www.semanticweb.org/patriciapoveda/ontologies/2020/4/ontology-place.owl#Weighing_Area"/>
        <owl:disjointWith rdf:resource="http://www.semanticweb.org/patriciapoveda/ontologies/2020/4/ontology-place.owl#Warehouse_Weighing_Area"/>
    </owl:Class>
    


    <!-- http://www.semanticweb.org/patriciapoveda/ontologies/2020/4/ontology-place.owl#Download -->

    <owl:Class rdf:about="http://www.semanticweb.org/patriciapoveda/ontologies/2020/4/ontology-place.owl#Download">
        <rdfs:subClassOf rdf:resource="http://www.semanticweb.org/patriciapoveda/ontologies/2020/4/ontology-place.owl#Logistics_Services"/>
        <rdfs:comment xml:lang="es">Esta clase sirve para recoger los productos que ya han completado el proceso y se encuentran en el almacén, para poder llevar un seguimiento de ellos.</rdfs:comment>
        <rdfs:comment xml:lang="en">This class is created to follow the products that have already completed the process and are in the warehouse, in order to keep track of them.</rdfs:comment>
    </owl:Class>
    


    <!-- http://www.semanticweb.org/patriciapoveda/ontologies/2020/4/ontology-place.owl#Download_Stop -->

    <owl:Class rdf:about="http://www.semanticweb.org/patriciapoveda/ontologies/2020/4/ontology-place.owl#Download_Stop">
        <rdfs:subClassOf rdf:resource="https://apiict01.etsii.upm.es/mediawiki/index.php/User:PatriciaPoveda/ontologia.owl#Stops_Inter-segment"/>
    </owl:Class>
    


    <!-- http://www.semanticweb.org/patriciapoveda/ontologies/2020/4/ontology-place.owl#Incidence_Stop -->

    <owl:Class rdf:about="http://www.semanticweb.org/patriciapoveda/ontologies/2020/4/ontology-place.owl#Incidence_Stop">
        <rdfs:subClassOf rdf:resource="https://apiict01.etsii.upm.es/mediawiki/index.php/User:PatriciaPoveda/ontologia.owl#Stops_Inter-segment"/>
    </owl:Class>
    


    <!-- http://www.semanticweb.org/patriciapoveda/ontologies/2020/4/ontology-place.owl#Load_Area -->

    <owl:Class rdf:about="http://www.semanticweb.org/patriciapoveda/ontologies/2020/4/ontology-place.owl#Load_Area">
        <rdfs:subClassOf rdf:resource="http://www.semanticweb.org/patriciapoveda/ontologies/2020/4/ontology-place.owl#Areas"/>
        <rdfs:comment xml:lang="en">Loading area for customers, intended for trucks to be positioned when loading. It is a limited area, for few vehicles at the same time. Trucks will have to wait outside to enter if they are fully occupied.</rdfs:comment>
        <rdfs:comment xml:lang="es">Área de carga para los clientes, destinada a que se posicionen los camiones al cargar. Zona muy limitada, para pocos vehículos a un mismo tiempo. Los camiones tendrán que esperar para entrar si esta ocupada al completo.</rdfs:comment>
    </owl:Class>
    


    <!-- http://www.semanticweb.org/patriciapoveda/ontologies/2020/4/ontology-place.owl#Logistics_Resources -->

    <owl:Class rdf:about="http://www.semanticweb.org/patriciapoveda/ontologies/2020/4/ontology-place.owl#Logistics_Resources">
        <rdfs:comment xml:lang="es">Esta clase principal incluye todos los recursos que se emplean a lo largo del proceso. Se refiere a elementos fisicos que se emplean para completar los procesos.</rdfs:comment>
        <rdfs:comment xml:lang="es">This main class includes all the resources that are used throughout the process. It makes reference to physical elements that are used to complete the processes.</rdfs:comment>
    </owl:Class>
    


    <!-- http://www.semanticweb.org/patriciapoveda/ontologies/2020/4/ontology-place.owl#Logistics_Services -->

    <owl:Class rdf:about="http://www.semanticweb.org/patriciapoveda/ontologies/2020/4/ontology-place.owl#Logistics_Services">
        <rdfs:comment xml:lang="es">Esta clase principal abarca los elementos no físicos que forman parte del proceso, sino los servicios o fases que tienen lugar a lo largo del sistema y que forman el proceso.</rdfs:comment>
        <rdfs:comment xml:lang="en">This main class covers the non-physical elements that are part of the process, like acts or phases that happens throughout the system.</rdfs:comment>
    </owl:Class>
    


    <!-- http://www.semanticweb.org/patriciapoveda/ontologies/2020/4/ontology-place.owl#Lunch_Stop -->

    <owl:Class rdf:about="http://www.semanticweb.org/patriciapoveda/ontologies/2020/4/ontology-place.owl#Lunch_Stop">
        <rdfs:subClassOf rdf:resource="https://apiict01.etsii.upm.es/mediawiki/index.php/User:PatriciaPoveda/ontologia.owl#Stops_Inter-segment"/>
    </owl:Class>
    


    <!-- http://www.semanticweb.org/patriciapoveda/ontologies/2020/4/ontology-place.owl#Pick-up_Stop -->

    <owl:Class rdf:about="http://www.semanticweb.org/patriciapoveda/ontologies/2020/4/ontology-place.owl#Pick-up_Stop">
        <rdfs:subClassOf rdf:resource="https://apiict01.etsii.upm.es/mediawiki/index.php/User:PatriciaPoveda/ontologia.owl#Stops_Inter-segment"/>
    </owl:Class>
    


    <!-- http://www.semanticweb.org/patriciapoveda/ontologies/2020/4/ontology-place.owl#Porters -->

    <owl:Class rdf:about="http://www.semanticweb.org/patriciapoveda/ontologies/2020/4/ontology-place.owl#Porters">
        <rdfs:subClassOf rdf:resource="http://www.semanticweb.org/patriciapoveda/ontologies/2020/4/ontology-place.owl#Supplier"/>
        <rdfs:comment xml:lang="es">Trabajadores encargados de cargar y descargar los productos para luego almacenarlos una vez los camiones han sido pesados. Se encargan además llevar el recuento de los materiales.</rdfs:comment>
        <rdfs:comment xml:lang="en">Workers that are in charge of loading and unloading the products and then storing them once the trucks have been weighed. They are also in charge of keeping count of the materials.</rdfs:comment>
    </owl:Class>
    


    <!-- http://www.semanticweb.org/patriciapoveda/ontologies/2020/4/ontology-place.owl#Product_Warehouse -->

    <owl:Class rdf:about="http://www.semanticweb.org/patriciapoveda/ontologies/2020/4/ontology-place.owl#Product_Warehouse">
        <rdfs:subClassOf rdf:resource="https://apiict01.etsii.upm.es/mediawiki/index.php/User:PatriciaPoveda/ontologia.owl#Warehouses"/>
        <rdfs:comment xml:lang="en">Destination set for each vehicle with the products they have collected on the routes, for the storage of the products until their subsequent recycling, reuse, incineration, etc.</rdfs:comment>
        <rdfs:comment xml:lang="es">Destino fijado para cada vehículo con los productos que se han recogido en las rutas, para el almacenamiento de los productos hasta su posterior reciclaje, reutilización, incineración, etc.</rdfs:comment>
    </owl:Class>
    


    <!-- http://www.semanticweb.org/patriciapoveda/ontologies/2020/4/ontology-place.owl#Real_Time_Location -->

    <owl:Class rdf:about="http://www.semanticweb.org/patriciapoveda/ontologies/2020/4/ontology-place.owl#Real_Time_Location">
        <rdfs:comment xml:lang="en">It collects real time positions of entities as vehicles, products, etc., throughout the different activities such as transport, weighing... Thanks to tools such as the timestamp and  GPS systems, it will be possible to know where the product is in the process and the exact location of the vehicle</rdfs:comment>
        <rdfs:comment xml:lang="es">Recoge las posiciones en tiempo real de los vehículos, productos, etc., a lo largo de las diferentes actividades como el transporte, la pesada, etc. Gracias a herramientas, por ejemplo, como el timestamp, se podrá saber en que parte del proceso esta el producto, y con sistemas GPS la localización exacta del vehículo</rdfs:comment>
    </owl:Class>
    


    <!-- http://www.semanticweb.org/patriciapoveda/ontologies/2020/4/ontology-place.owl#Scale -->

    <owl:Class rdf:about="http://www.semanticweb.org/patriciapoveda/ontologies/2020/4/ontology-place.owl#Scale">
        <rdfs:subClassOf rdf:resource="http://www.semanticweb.org/patriciapoveda/ontologies/2020/4/ontology-place.owl#Logistics_Resources"/>
        <rdfs:comment xml:lang="es">Clase para las básculas que recogen los pesos de vehículos en las entradas y salidas de los locales de los clientes y los almacenes, para con la diferencia de pesos entre entrada y salida calcular y comprobar el peso del material.</rdfs:comment>
        <rdfs:comment xml:lang="en">Class for scales that collect vehicle weights at the entrances and exits of customer premises and warehouses, to calculate and check the weight of the material thanks to the difference  between entry and exit weights.</rdfs:comment>
    </owl:Class>
    


    <!-- http://www.semanticweb.org/patriciapoveda/ontologies/2020/4/ontology-place.owl#Scheduling -->

    <owl:Class rdf:about="http://www.semanticweb.org/patriciapoveda/ontologies/2020/4/ontology-place.owl#Scheduling">
        <rdfs:subClassOf rdf:resource="http://www.semanticweb.org/patriciapoveda/ontologies/2020/4/ontology-place.owl#Activities"/>
    </owl:Class>
    


    <!-- http://www.semanticweb.org/patriciapoveda/ontologies/2020/4/ontology-place.owl#Stop -->

    <owl:Class rdf:about="http://www.semanticweb.org/patriciapoveda/ontologies/2020/4/ontology-place.owl#Stop">
        <owl:equivalentClass rdf:resource="https://apiict01.etsii.upm.es/mediawiki/index.php/User:PatriciaPoveda/ontologia.owl#Stops_Inter-segment"/>
        <rdfs:subClassOf rdf:resource="http://www.semanticweb.org/patriciapoveda/ontologies/2020/4/ontology-place.owl#Activities"/>
    </owl:Class>
    


    <!-- http://www.semanticweb.org/patriciapoveda/ontologies/2020/4/ontology-place.owl#Storage -->

    <owl:Class rdf:about="http://www.semanticweb.org/patriciapoveda/ontologies/2020/4/ontology-place.owl#Storage">
        <rdfs:subClassOf rdf:resource="http://www.semanticweb.org/patriciapoveda/ontologies/2020/4/ontology-place.owl#Activities"/>
    </owl:Class>
    


    <!-- http://www.semanticweb.org/patriciapoveda/ontologies/2020/4/ontology-place.owl#Sup.Manager -->

    <owl:Class rdf:about="http://www.semanticweb.org/patriciapoveda/ontologies/2020/4/ontology-place.owl#Sup.Manager">
        <rdfs:subClassOf rdf:resource="http://www.semanticweb.org/patriciapoveda/ontologies/2020/4/ontology-place.owl#Supplier"/>
        <rdfs:comment xml:lang="en">People in charge of leading the process from the suppliers&apos; position, leading the suppliers team and making decisions</rdfs:comment>
        <rdfs:comment xml:lang="es">Personas encargadas de dirigir el proceso desde la posición de los proveedores, dirigiendo a los basculistas, mozos y conductores y tomando decisiones.</rdfs:comment>
    </owl:Class>
    


    <!-- http://www.semanticweb.org/patriciapoveda/ontologies/2020/4/ontology-place.owl#Sup.Weighing_Worker -->

    <owl:Class rdf:about="http://www.semanticweb.org/patriciapoveda/ontologies/2020/4/ontology-place.owl#Sup.Weighing_Worker">
        <rdfs:subClassOf rdf:resource="http://www.semanticweb.org/patriciapoveda/ontologies/2020/4/ontology-place.owl#Supplier"/>
        <rdfs:comment xml:lang="en">People that are in charge of weighing the product when the truck is going to unload it in the warehouse, weighing the truck when it is entering and leaving the warehouse to calculate the load difference.</rdfs:comment>
        <rdfs:comment xml:lang="es">Personas encargadas de pesar el producto cuando el camión va a descargar en el almacén, pesando el camión al entrar y al salir para calcular la diferencia de carga.</rdfs:comment>
    </owl:Class>
    


    <!-- http://www.semanticweb.org/patriciapoveda/ontologies/2020/4/ontology-place.owl#Supplier -->

    <owl:Class rdf:about="http://www.semanticweb.org/patriciapoveda/ontologies/2020/4/ontology-place.owl#Supplier">
        <rdfs:subClassOf rdf:resource="https://apiict01.etsii.upm.es/mediawiki/index.php/User:PatriciaPoveda/ontologia.owl#Agents"/>
        <rdfs:comment xml:lang="en">Person or entity that wants to get the product that the customer is sells and is in charge of the transport process to pick it up.</rdfs:comment>
        <rdfs:comment xml:lang="es">Persona o entidad que quiere hacerse con el producto que vende el cliente y se encarga del proceso de transporte que implica ir a recogerlo.</rdfs:comment>
    </owl:Class>
    


    <!-- http://www.semanticweb.org/patriciapoveda/ontologies/2020/4/ontology-place.owl#Transport -->

    <owl:Class rdf:about="http://www.semanticweb.org/patriciapoveda/ontologies/2020/4/ontology-place.owl#Transport">
        <rdfs:subClassOf rdf:resource="http://www.semanticweb.org/patriciapoveda/ontologies/2020/4/ontology-place.owl#Activities"/>
    </owl:Class>
    


    <!-- http://www.semanticweb.org/patriciapoveda/ontologies/2020/4/ontology-place.owl#Vehicle_Garage -->

    <owl:Class rdf:about="http://www.semanticweb.org/patriciapoveda/ontologies/2020/4/ontology-place.owl#Vehicle_Garage">
        <rdfs:subClassOf rdf:resource="https://apiict01.etsii.upm.es/mediawiki/index.php/User:PatriciaPoveda/ontologia.owl#Warehouses"/>
        <rdfs:comment xml:lang="es">Lugar de partida de los vehículos donde se encuentran aparcados hasta que se les destina a una ruta.</rdfs:comment>
        <rdfs:comment xml:lang="en">Starting point of the route where the vehicles are parked until they are assigned to a route.</rdfs:comment>
    </owl:Class>
    


    <!-- http://www.semanticweb.org/patriciapoveda/ontologies/2020/4/ontology-place.owl#W_Scale_Entry -->

    <owl:Class rdf:about="http://www.semanticweb.org/patriciapoveda/ontologies/2020/4/ontology-place.owl#W_Scale_Entry">
        <rdfs:subClassOf rdf:resource="http://www.semanticweb.org/patriciapoveda/ontologies/2020/4/ontology-place.owl#Warehouse_Scale"/>
    </owl:Class>
    


    <!-- http://www.semanticweb.org/patriciapoveda/ontologies/2020/4/ontology-place.owl#W_Scale_Exit -->

    <owl:Class rdf:about="http://www.semanticweb.org/patriciapoveda/ontologies/2020/4/ontology-place.owl#W_Scale_Exit">
        <rdfs:subClassOf rdf:resource="http://www.semanticweb.org/patriciapoveda/ontologies/2020/4/ontology-place.owl#Warehouse_Scale"/>
    </owl:Class>
    


    <!-- http://www.semanticweb.org/patriciapoveda/ontologies/2020/4/ontology-place.owl#Warehouse_Scale -->

    <owl:Class rdf:about="http://www.semanticweb.org/patriciapoveda/ontologies/2020/4/ontology-place.owl#Warehouse_Scale">
        <rdfs:subClassOf rdf:resource="http://www.semanticweb.org/patriciapoveda/ontologies/2020/4/ontology-place.owl#Scale"/>
    </owl:Class>
    


    <!-- http://www.semanticweb.org/patriciapoveda/ontologies/2020/4/ontology-place.owl#Warehouse_Storage_Area -->

    <owl:Class rdf:about="http://www.semanticweb.org/patriciapoveda/ontologies/2020/4/ontology-place.owl#Warehouse_Storage_Area">
        <rdfs:subClassOf rdf:resource="https://apiict01.etsii.upm.es/mediawiki/index.php/User:PatriciaPoveda/ontologia.owl#Storage_Area"/>
    </owl:Class>
    


    <!-- http://www.semanticweb.org/patriciapoveda/ontologies/2020/4/ontology-place.owl#Warehouse_Weighing_Area -->

    <owl:Class rdf:about="http://www.semanticweb.org/patriciapoveda/ontologies/2020/4/ontology-place.owl#Warehouse_Weighing_Area">
        <rdfs:subClassOf rdf:resource="http://www.semanticweb.org/patriciapoveda/ontologies/2020/4/ontology-place.owl#Weighing_Area"/>
    </owl:Class>
    


    <!-- http://www.semanticweb.org/patriciapoveda/ontologies/2020/4/ontology-place.owl#Weighing -->

    <owl:Class rdf:about="http://www.semanticweb.org/patriciapoveda/ontologies/2020/4/ontology-place.owl#Weighing">
        <rdfs:subClassOf rdf:resource="https://apiict01.etsii.upm.es/mediawiki/index.php/User:PatriciaPoveda/ontologia.owl#Stops_Inter-segment"/>
    </owl:Class>
    


    <!-- http://www.semanticweb.org/patriciapoveda/ontologies/2020/4/ontology-place.owl#Weighing_Area -->

    <owl:Class rdf:about="http://www.semanticweb.org/patriciapoveda/ontologies/2020/4/ontology-place.owl#Weighing_Area">
        <rdfs:subClassOf rdf:resource="http://www.semanticweb.org/patriciapoveda/ontologies/2020/4/ontology-place.owl#Areas"/>
        <rdfs:comment xml:lang="en">Area where trucks are weighed, when entering and leaving the palce to calculate the weight of the material that has been picked up</rdfs:comment>
        <rdfs:comment xml:lang="es">Área donde se pesan los camiones, al entrar y al salir para calcular el peso del material.</rdfs:comment>
    </owl:Class>
    


    <!-- http://www.w3.org/2002/07/owl#Thing -->

    <owl:Class rdf:about="http://www.w3.org/2002/07/owl#Thing"/>
    


    <!-- https://apiict01.etsii.upm.es/mediawiki/index.php/User:PatriciaPoveda/ontologia.owl#Agents -->

    <owl:Class rdf:about="https://apiict01.etsii.upm.es/mediawiki/index.php/User:PatriciaPoveda/ontologia.owl#Agents">
        <rdfs:subClassOf rdf:resource="http://www.semanticweb.org/patriciapoveda/ontologies/2020/4/ontology-place.owl#Logistics_Resources"/>
        <rdfs:comment xml:lang="en">Logistics agents are individuals or legal entities created for commercial ventures. To model these entities, we consider how they participate in the  supply chains system.</rdfs:comment>
        <rdfs:comment xml:lang="es">Los agentes de logística son individuos o actores corporativos, es decir, entidades legales creadas para emprendimientos comerciales. Para situarles en el modelo, consideramos la forma en que participan en las cadenas de suministro.</rdfs:comment>
    </owl:Class>
    


    <!-- https://apiict01.etsii.upm.es/mediawiki/index.php/User:PatriciaPoveda/ontologia.owl#Customer -->

    <owl:Class rdf:about="https://apiict01.etsii.upm.es/mediawiki/index.php/User:PatriciaPoveda/ontologia.owl#Customer">
        <rdfs:subClassOf rdf:resource="https://apiict01.etsii.upm.es/mediawiki/index.php/User:PatriciaPoveda/ontologia.owl#Agents"/>
        <rdfs:comment xml:lang="en">Legal or natural person who ask for the service</rdfs:comment>
        <rdfs:comment xml:lang="es">Persona juridica o fisica que hace el encargo</rdfs:comment>
    </owl:Class>
    


    <!-- https://apiict01.etsii.upm.es/mediawiki/index.php/User:PatriciaPoveda/ontologia.owl#Download_Area -->

    <owl:Class rdf:about="https://apiict01.etsii.upm.es/mediawiki/index.php/User:PatriciaPoveda/ontologia.owl#Download_Area">
        <rdfs:subClassOf rdf:resource="http://www.semanticweb.org/patriciapoveda/ontologies/2020/4/ontology-place.owl#Areas"/>
        <rdfs:comment xml:lang="en">Warehouse dowloading area, where the trucks are positioned when downloading the material. Limited area, for a few vehicules at the same time. Trucks will have to wait outside to enter if it is fully occupied.</rdfs:comment>
        <rdfs:comment xml:lang="es">Área de descarga de los almacenes, destinada a que se posicionen los camiones al descragar. Zona muy limitada, para pocos vehiculos a un mismo tiempo. Los camiones tendran que esperar para entrar si esta ocupada al completo</rdfs:comment>
    </owl:Class>
    


    <!-- https://apiict01.etsii.upm.es/mediawiki/index.php/User:PatriciaPoveda/ontologia.owl#Driver -->

    <owl:Class rdf:about="https://apiict01.etsii.upm.es/mediawiki/index.php/User:PatriciaPoveda/ontologia.owl#Driver">
        <rdfs:subClassOf rdf:resource="http://www.semanticweb.org/patriciapoveda/ontologies/2020/4/ontology-place.owl#Supplier"/>
        <rdfs:comment xml:lang="es">Trabajadores que conducen los vehiculos y cumplen con las rutas establecidas.</rdfs:comment>
        <rdfs:comment xml:lang="en">Workers who drive the vehicles and fulfill with the established routes.</rdfs:comment>
    </owl:Class>
    


    <!-- https://apiict01.etsii.upm.es/mediawiki/index.php/User:PatriciaPoveda/ontologia.owl#HydraulicCrane -->

    <owl:Class rdf:about="https://apiict01.etsii.upm.es/mediawiki/index.php/User:PatriciaPoveda/ontologia.owl#HydraulicCrane">
        <rdfs:subClassOf rdf:resource="https://apiict01.etsii.upm.es/mediawiki/index.php/User:PatriciaPoveda/ontologia.owl#Truck_Crane"/>
    </owl:Class>
    


    <!-- https://apiict01.etsii.upm.es/mediawiki/index.php/User:PatriciaPoveda/ontologia.owl#JibCrane -->

    <owl:Class rdf:about="https://apiict01.etsii.upm.es/mediawiki/index.php/User:PatriciaPoveda/ontologia.owl#JibCrane">
        <rdfs:subClassOf rdf:resource="https://apiict01.etsii.upm.es/mediawiki/index.php/User:PatriciaPoveda/ontologia.owl#Truck_Crane"/>
    </owl:Class>
    


    <!-- https://apiict01.etsii.upm.es/mediawiki/index.php/User:PatriciaPoveda/ontologia.owl#OctopusCrane -->

    <owl:Class rdf:about="https://apiict01.etsii.upm.es/mediawiki/index.php/User:PatriciaPoveda/ontologia.owl#OctopusCrane">
        <rdfs:subClassOf rdf:resource="https://apiict01.etsii.upm.es/mediawiki/index.php/User:PatriciaPoveda/ontologia.owl#Truck_Crane"/>
    </owl:Class>
    


    <!-- https://apiict01.etsii.upm.es/mediawiki/index.php/User:PatriciaPoveda/ontologia.owl#Product -->

    <owl:Class rdf:about="https://apiict01.etsii.upm.es/mediawiki/index.php/User:PatriciaPoveda/ontologia.owl#Product">
        <rdfs:subClassOf rdf:resource="http://www.semanticweb.org/patriciapoveda/ontologies/2020/4/ontology-place.owl#Logistics_Resources"/>
        <rdfs:comment xml:lang="es">Materiales que se van a recoger. Son materiales metálicos, de distintas dimensiones y pesos.
Los materiales se recogen con el objetivo de darles un tratamiento posterior: reciclaje, reutilizacion, eliminación...</rdfs:comment>
        <rdfs:comment xml:lang="en">Materials to be collected. They are metallic materials with different dimensions and weights.</rdfs:comment>
    </owl:Class>
    


    <!-- https://apiict01.etsii.upm.es/mediawiki/index.php/User:PatriciaPoveda/ontologia.owl#Segments -->

    <owl:Class rdf:about="https://apiict01.etsii.upm.es/mediawiki/index.php/User:PatriciaPoveda/ontologia.owl#Segments">
        <rdfs:subClassOf rdf:resource="http://www.semanticweb.org/patriciapoveda/ontologies/2020/4/ontology-place.owl#Logistics_Services"/>
        <rdfs:comment xml:lang="es">Secciones que componen la ruta separadas por las distintas paradas (puntos de recogida)</rdfs:comment>
        <rdfs:comment xml:lang="en">Segements that make up the route, they are separated by the different stops (pick up points)</rdfs:comment>
    </owl:Class>
    


    <!-- https://apiict01.etsii.upm.es/mediawiki/index.php/User:PatriciaPoveda/ontologia.owl#Sidelifter -->

    <owl:Class rdf:about="https://apiict01.etsii.upm.es/mediawiki/index.php/User:PatriciaPoveda/ontologia.owl#Sidelifter">
        <rdfs:subClassOf rdf:resource="https://apiict01.etsii.upm.es/mediawiki/index.php/User:PatriciaPoveda/ontologia.owl#Truck_Crane"/>
    </owl:Class>
    


    <!-- https://apiict01.etsii.upm.es/mediawiki/index.php/User:PatriciaPoveda/ontologia.owl#Stops_Inter-segment -->

    <owl:Class rdf:about="https://apiict01.etsii.upm.es/mediawiki/index.php/User:PatriciaPoveda/ontologia.owl#Stops_Inter-segment">
        <rdfs:subClassOf rdf:resource="http://www.semanticweb.org/patriciapoveda/ontologies/2020/4/ontology-place.owl#Logistics_Services"/>
        <rdfs:comment xml:lang="es">Paradas en las diferentes rutas, corresponden con los puntos de recogida de los productos, en los locales de los clientes.</rdfs:comment>
        <rdfs:comment xml:lang="en">Stops on the different routes. They are the pick up points of the products,  the clients&apos; adresses.</rdfs:comment>
    </owl:Class>
    


    <!-- https://apiict01.etsii.upm.es/mediawiki/index.php/User:PatriciaPoveda/ontologia.owl#Storage_Area -->

    <owl:Class rdf:about="https://apiict01.etsii.upm.es/mediawiki/index.php/User:PatriciaPoveda/ontologia.owl#Storage_Area">
        <rdfs:subClassOf rdf:resource="http://www.semanticweb.org/patriciapoveda/ontologies/2020/4/ontology-place.owl#Areas"/>
        <rdfs:comment xml:lang="en">Materials storage area, where the products are stored until further processing. Limited area but with large capacity</rdfs:comment>
        <rdfs:comment xml:lang="es">Área de almacenamiento de los materiales, donde se guardan hasta su posterior proceso. Zona limitada pero con gran capacidad</rdfs:comment>
    </owl:Class>
    


    <!-- https://apiict01.etsii.upm.es/mediawiki/index.php/User:PatriciaPoveda/ontologia.owl#TelescopicCrane -->

    <owl:Class rdf:about="https://apiict01.etsii.upm.es/mediawiki/index.php/User:PatriciaPoveda/ontologia.owl#TelescopicCrane">
        <rdfs:subClassOf rdf:resource="https://apiict01.etsii.upm.es/mediawiki/index.php/User:PatriciaPoveda/ontologia.owl#Truck_Crane"/>
    </owl:Class>
    


    <!-- https://apiict01.etsii.upm.es/mediawiki/index.php/User:PatriciaPoveda/ontologia.owl#Trajectory -->

    <owl:Class rdf:about="https://apiict01.etsii.upm.es/mediawiki/index.php/User:PatriciaPoveda/ontologia.owl#Trajectory">
        <rdfs:subClassOf rdf:resource="http://www.semanticweb.org/patriciapoveda/ontologies/2020/4/ontology-place.owl#Logistics_Services"/>
        <rdfs:subClassOf>
            <owl:Class>
                <owl:intersectionOf rdf:parseType="Collection">
                    <rdf:Description rdf:about="https://apiict01.etsii.upm.es/mediawiki/index.php/User:PatriciaPoveda/ontologia.owl#Segments"/>
                    <rdf:Description rdf:about="https://apiict01.etsii.upm.es/mediawiki/index.php/User:PatriciaPoveda/ontologia.owl#Stops_Inter-segment"/>
                </owl:intersectionOf>
            </owl:Class>
        </rdfs:subClassOf>
        <rdfs:comment xml:lang="es">Recorridos (rutas) que van a seguir los diferentes vehiculos, desde el lugar del que parten, pasando por los distintos clientes incluidos en su recorrido hasta el lugar de almacenamiento final y volviendo al garaje de los vehiculos.
 Para la determinación de las rutas habrá que tener en cuenta el trafico en tiempo real, y los kilómetros y duración de la misma para seleccionar los vehículos asignados a cada una de ellas. Las rutas tendrán diferentes paradas.</rdfs:comment>
        <rdfs:comment xml:lang="en">Routes that the different vehicles have to follow,  beginning in the place where the vehicules are parked passing through the different clients included in their route to the final storage location and returning to the vehicle garage.
When deciding the routes it will be necessary to take into account the real time traffic. The routes will have different stops.</rdfs:comment>
    </owl:Class>
    


    <!-- https://apiict01.etsii.upm.es/mediawiki/index.php/User:PatriciaPoveda/ontologia.owl#Truck_Box -->

    <owl:Class rdf:about="https://apiict01.etsii.upm.es/mediawiki/index.php/User:PatriciaPoveda/ontologia.owl#Truck_Box">
        <rdfs:subClassOf rdf:resource="https://apiict01.etsii.upm.es/mediawiki/index.php/User:PatriciaPoveda/ontologia.owl#Vehicle"/>
    </owl:Class>
    


    <!-- https://apiict01.etsii.upm.es/mediawiki/index.php/User:PatriciaPoveda/ontologia.owl#Truck_Crane -->

    <owl:Class rdf:about="https://apiict01.etsii.upm.es/mediawiki/index.php/User:PatriciaPoveda/ontologia.owl#Truck_Crane">
        <rdfs:subClassOf rdf:resource="https://apiict01.etsii.upm.es/mediawiki/index.php/User:PatriciaPoveda/ontologia.owl#Vehicle"/>
    </owl:Class>
    


    <!-- https://apiict01.etsii.upm.es/mediawiki/index.php/User:PatriciaPoveda/ontologia.owl#Truck_Hopper -->

    <owl:Class rdf:about="https://apiict01.etsii.upm.es/mediawiki/index.php/User:PatriciaPoveda/ontologia.owl#Truck_Hopper">
        <rdfs:subClassOf rdf:resource="https://apiict01.etsii.upm.es/mediawiki/index.php/User:PatriciaPoveda/ontologia.owl#Vehicle"/>
    </owl:Class>
    


    <!-- https://apiict01.etsii.upm.es/mediawiki/index.php/User:PatriciaPoveda/ontologia.owl#Truck_Platform -->

    <owl:Class rdf:about="https://apiict01.etsii.upm.es/mediawiki/index.php/User:PatriciaPoveda/ontologia.owl#Truck_Platform">
        <rdfs:subClassOf rdf:resource="https://apiict01.etsii.upm.es/mediawiki/index.php/User:PatriciaPoveda/ontologia.owl#Vehicle"/>
    </owl:Class>
    


    <!-- https://apiict01.etsii.upm.es/mediawiki/index.php/User:PatriciaPoveda/ontologia.owl#Truck_Tipper_Bus -->

    <owl:Class rdf:about="https://apiict01.etsii.upm.es/mediawiki/index.php/User:PatriciaPoveda/ontologia.owl#Truck_Tipper_Bus">
        <rdfs:subClassOf rdf:resource="https://apiict01.etsii.upm.es/mediawiki/index.php/User:PatriciaPoveda/ontologia.owl#Vehicle"/>
    </owl:Class>
    


    <!-- https://apiict01.etsii.upm.es/mediawiki/index.php/User:PatriciaPoveda/ontologia.owl#Van -->

    <owl:Class rdf:about="https://apiict01.etsii.upm.es/mediawiki/index.php/User:PatriciaPoveda/ontologia.owl#Van">
        <rdfs:subClassOf rdf:resource="https://apiict01.etsii.upm.es/mediawiki/index.php/User:PatriciaPoveda/ontologia.owl#Vehicle"/>
    </owl:Class>
    


    <!-- https://apiict01.etsii.upm.es/mediawiki/index.php/User:PatriciaPoveda/ontologia.owl#Vehicle -->

    <owl:Class rdf:about="https://apiict01.etsii.upm.es/mediawiki/index.php/User:PatriciaPoveda/ontologia.owl#Vehicle">
        <rdfs:subClassOf rdf:resource="http://www.semanticweb.org/patriciapoveda/ontologies/2020/4/ontology-place.owl#Logistics_Resources"/>
        <rdfs:comment xml:lang="es">Clase que recoge los diferentes tipos de vehiculos que forman la flota.
Los vehículos son de distintos tipos, dimensiones y capacidades de carga para adaptarse a las distintas dimensiones y características de los productos. Según esto se asignará uno u otro a cada encargo.</rdfs:comment>
        <rdfs:comment xml:lang="en">Class that includes the different types of vehicles the fleet is composed by.
Vehicles are of different types, dimensions and load capacities, in order to adapt to the different dimensions and characteristics of the products. According to that, one or another will be assigned to each assignment.</rdfs:comment>
    </owl:Class>
    


    <!-- https://apiict01.etsii.upm.es/mediawiki/index.php/User:PatriciaPoveda/ontologia.owl#Warehouses -->

    <owl:Class rdf:about="https://apiict01.etsii.upm.es/mediawiki/index.php/User:PatriciaPoveda/ontologia.owl#Warehouses">
        <rdfs:subClassOf rdf:resource="http://www.semanticweb.org/patriciapoveda/ontologies/2020/4/ontology-place.owl#Logistics_Resources"/>
        <rdfs:comment xml:lang="es">Almacenes de productos o de vehiculos</rdfs:comment>
        <rdfs:comment xml:lang="en">Warehouses of products or vehicles</rdfs:comment>
    </owl:Class>
    


    <!-- 
    ///////////////////////////////////////////////////////////////////////////////////////
    //
    // Individuals
    //
    ///////////////////////////////////////////////////////////////////////////////////////
     -->

    


    <!-- http://www.semanticweb.org/patriciapoveda/ontologies/2020/4/ontology-place.owl#Almacen1 -->

    <owl:NamedIndividual rdf:about="http://www.semanticweb.org/patriciapoveda/ontologies/2020/4/ontology-place.owl#Almacen1">
        <rdf:type rdf:resource="http://www.semanticweb.org/patriciapoveda/ontologies/2020/4/ontology-place.owl#Product_Warehouse"/>
        <place:is_located_in rdf:resource="http://www.semanticweb.org/patriciapoveda/ontologies/2020/4/ontology-place.owl#PlaceX"/>
        <ontology-place:has_opening_hours rdf:resource="http://www.semanticweb.org/patriciapoveda/ontologies/2020/4/ontology-place.owl#TimeAlmacén1"/>
        <ontology-place:is_destination_of rdf:resource="http://www.semanticweb.org/patriciapoveda/ontologies/2020/4/ontology-place.owl#Route1"/>
        <ontologia:Store rdf:resource="http://www.semanticweb.org/patriciapoveda/ontologies/2020/4/ontology-place.owl#Product1"/>
        <ontology-place:Occupation_Level rdf:datatype="http://www.w3.org/2001/XMLSchema#string">20%</ontology-place:Occupation_Level>
        <ontologia:Adress_Warehouse>Alcorcón</ontologia:Adress_Warehouse>
        <ontologia:Capac_Warehouse rdf:datatype="http://www.w3.org/2001/XMLSchema#float">1000.0</ontologia:Capac_Warehouse>
    </owl:NamedIndividual>
    


    <!-- http://www.semanticweb.org/patriciapoveda/ontologies/2020/4/ontology-place.owl#Camion1 -->

    <owl:NamedIndividual rdf:about="http://www.semanticweb.org/patriciapoveda/ontologies/2020/4/ontology-place.owl#Camion1">
        <rdf:type rdf:resource="https://apiict01.etsii.upm.es/mediawiki/index.php/User:PatriciaPoveda/ontologia.owl#Van"/>
    </owl:NamedIndividual>
    


    <!-- http://www.semanticweb.org/patriciapoveda/ontologies/2020/4/ontology-place.owl#Cliente1 -->

    <owl:NamedIndividual rdf:about="http://www.semanticweb.org/patriciapoveda/ontologies/2020/4/ontology-place.owl#Cliente1">
        <rdf:type rdf:resource="http://www.semanticweb.org/patriciapoveda/ontologies/2020/4/ontology-place.owl#Cust.Manager"/>
        <ontology-place:has_time_slot rdf:resource="http://www.semanticweb.org/patriciapoveda/ontologies/2020/4/ontology-place.owl#TimeCliente1"/>
        <ontology-place:is_included rdf:resource="http://www.semanticweb.org/patriciapoveda/ontologies/2020/4/ontology-place.owl#Route1"/>
        <ontologia:Owns rdf:resource="http://www.semanticweb.org/patriciapoveda/ontologies/2020/4/ontology-place.owl#Product1"/>
        <ontologia:Adress_Customer>Madrid</ontologia:Adress_Customer>
        <ontologia:ID_Customer>01</ontologia:ID_Customer>
        <ontologia:Name>Juan</ontologia:Name>
    </owl:NamedIndividual>
    


    <!-- http://www.semanticweb.org/patriciapoveda/ontologies/2020/4/ontology-place.owl#Driver1 -->

    <owl:NamedIndividual rdf:about="http://www.semanticweb.org/patriciapoveda/ontologies/2020/4/ontology-place.owl#Driver1">
        <rdf:type rdf:resource="https://apiict01.etsii.upm.es/mediawiki/index.php/User:PatriciaPoveda/ontologia.owl#Driver"/>
        <ontologia:Is_driver_of rdf:resource="http://www.semanticweb.org/patriciapoveda/ontologies/2020/4/ontology-place.owl#Camion1"/>
        <ontologia:Experience>High</ontologia:Experience>
        <ontologia:ID_Supplier>020</ontologia:ID_Supplier>
        <ontologia:Name>Pedro</ontologia:Name>
        <ontologia:State>Busy</ontologia:State>
    </owl:NamedIndividual>
    


    <!-- http://www.semanticweb.org/patriciapoveda/ontologies/2020/4/ontology-place.owl#Garage1 -->

    <owl:NamedIndividual rdf:about="http://www.semanticweb.org/patriciapoveda/ontologies/2020/4/ontology-place.owl#Garage1">
        <rdf:type rdf:resource="http://www.semanticweb.org/patriciapoveda/ontologies/2020/4/ontology-place.owl#Vehicle_Garage"/>
        <ontology-place:is_ended_point_of rdf:resource="http://www.semanticweb.org/patriciapoveda/ontologies/2020/4/ontology-place.owl#Route1"/>
        <ontology-place:is_started_point_of rdf:resource="http://www.semanticweb.org/patriciapoveda/ontologies/2020/4/ontology-place.owl#Route1"/>
        <ontology-place:is_the_park_of rdf:resource="http://www.semanticweb.org/patriciapoveda/ontologies/2020/4/ontology-place.owl#Camion1"/>
    </owl:NamedIndividual>
    


    <!-- http://www.semanticweb.org/patriciapoveda/ontologies/2020/4/ontology-place.owl#PlaceX -->

    <owl:NamedIndividual rdf:about="http://www.semanticweb.org/patriciapoveda/ontologies/2020/4/ontology-place.owl#PlaceX">
        <rdf:type rdf:resource="http://www.ontologydesignpatterns.org/cp/owl/place.owl#Place"/>
    </owl:NamedIndividual>
    


    <!-- http://www.semanticweb.org/patriciapoveda/ontologies/2020/4/ontology-place.owl#Product1 -->

    <owl:NamedIndividual rdf:about="http://www.semanticweb.org/patriciapoveda/ontologies/2020/4/ontology-place.owl#Product1">
        <rdf:type rdf:resource="https://apiict01.etsii.upm.es/mediawiki/index.php/User:PatriciaPoveda/ontologia.owl#Product"/>
        <ontologia:Belongs_to rdf:resource="http://www.semanticweb.org/patriciapoveda/ontologies/2020/4/ontology-place.owl#Cliente1"/>
        <ontologia:Is_stored_by rdf:resource="http://www.semanticweb.org/patriciapoveda/ontologies/2020/4/ontology-place.owl#Almacen1"/>
        <ontologia:Is_transported_by rdf:resource="http://www.semanticweb.org/patriciapoveda/ontologies/2020/4/ontology-place.owl#Camion1"/>
        <ontology-place:Nature_of_material rdf:datatype="http://www.w3.org/2001/XMLSchema#string">Acero inoxidable</ontology-place:Nature_of_material>
        <ontology-place:Quality_Level_of_Material rdf:datatype="http://www.w3.org/2001/XMLSchema#string">High</ontology-place:Quality_Level_of_Material>
        <ontologia:Dimension rdf:datatype="http://www.w3.org/2001/XMLSchema#string">2 metros de ancho, 3 de largo y 1 de alto</ontologia:Dimension>
        <ontologia:Identifier rdf:datatype="http://www.w3.org/2001/XMLSchema#string">A1111</ontologia:Identifier>
        <ontologia:Load rdf:datatype="http://www.w3.org/2001/XMLSchema#string">10kg</ontologia:Load>
    </owl:NamedIndividual>
    


    <!-- http://www.semanticweb.org/patriciapoveda/ontologies/2020/4/ontology-place.owl#Route1 -->

    <owl:NamedIndividual rdf:about="http://www.semanticweb.org/patriciapoveda/ontologies/2020/4/ontology-place.owl#Route1">
        <rdf:type rdf:resource="https://apiict01.etsii.upm.es/mediawiki/index.php/User:PatriciaPoveda/ontologia.owl#Trajectory"/>
        <ontology-place:has rdf:resource="http://www.semanticweb.org/patriciapoveda/ontologies/2020/4/ontology-place.owl#Stop1"/>
        <ontology-place:has rdf:resource="http://www.semanticweb.org/patriciapoveda/ontologies/2020/4/ontology-place.owl#Stop2"/>
        <ontology-place:has rdf:resource="http://www.semanticweb.org/patriciapoveda/ontologies/2020/4/ontology-place.owl#Stop3"/>
        <ontology-place:has_end_point_in rdf:resource="http://www.semanticweb.org/patriciapoveda/ontologies/2020/4/ontology-place.owl#Garage1"/>
        <ontology-place:has_start_point_in rdf:resource="http://www.semanticweb.org/patriciapoveda/ontologies/2020/4/ontology-place.owl#Garage1"/>
        <ontologia:Path_Length rdf:datatype="http://www.w3.org/2001/XMLSchema#string">50km</ontologia:Path_Length>
        <ontologia:Path_Stops rdf:datatype="http://www.w3.org/2001/XMLSchema#integer">3</ontologia:Path_Stops>
        <ontologia:Traffic rdf:datatype="http://www.w3.org/2001/XMLSchema#string">Low</ontologia:Traffic>
    </owl:NamedIndividual>
    


    <!-- http://www.semanticweb.org/patriciapoveda/ontologies/2020/4/ontology-place.owl#Scale1 -->

    <owl:NamedIndividual rdf:about="http://www.semanticweb.org/patriciapoveda/ontologies/2020/4/ontology-place.owl#Scale1">
        <rdf:type rdf:resource="http://www.semanticweb.org/patriciapoveda/ontologies/2020/4/ontology-place.owl#Scale"/>
        <ontology-place:weighs rdf:resource="http://www.semanticweb.org/patriciapoveda/ontologies/2020/4/ontology-place.owl#Product1"/>
    </owl:NamedIndividual>
    


    <!-- http://www.semanticweb.org/patriciapoveda/ontologies/2020/4/ontology-place.owl#Stop1 -->

    <owl:NamedIndividual rdf:about="http://www.semanticweb.org/patriciapoveda/ontologies/2020/4/ontology-place.owl#Stop1">
        <rdf:type rdf:resource="http://www.semanticweb.org/patriciapoveda/ontologies/2020/4/ontology-place.owl#Stop"/>
        <ontology-place:happen_in rdf:resource="http://www.semanticweb.org/patriciapoveda/ontologies/2020/4/ontology-place.owl#Route1"/>
        <ontology-place:last rdf:resource="http://www.semanticweb.org/patriciapoveda/ontologies/2020/4/ontology-place.owl#TimeStop1"/>
    </owl:NamedIndividual>
    


    <!-- http://www.semanticweb.org/patriciapoveda/ontologies/2020/4/ontology-place.owl#Stop2 -->

    <owl:NamedIndividual rdf:about="http://www.semanticweb.org/patriciapoveda/ontologies/2020/4/ontology-place.owl#Stop2">
        <rdf:type rdf:resource="https://apiict01.etsii.upm.es/mediawiki/index.php/User:PatriciaPoveda/ontologia.owl#Stops_Inter-segment"/>
        <ontology-place:happen_in rdf:resource="http://www.semanticweb.org/patriciapoveda/ontologies/2020/4/ontology-place.owl#Route1"/>
        <ontology-place:last rdf:resource="http://www.semanticweb.org/patriciapoveda/ontologies/2020/4/ontology-place.owl#TimeStop2"/>
    </owl:NamedIndividual>
    


    <!-- http://www.semanticweb.org/patriciapoveda/ontologies/2020/4/ontology-place.owl#Stop3 -->

    <owl:NamedIndividual rdf:about="http://www.semanticweb.org/patriciapoveda/ontologies/2020/4/ontology-place.owl#Stop3">
        <rdf:type rdf:resource="https://apiict01.etsii.upm.es/mediawiki/index.php/User:PatriciaPoveda/ontologia.owl#Stops_Inter-segment"/>
        <ontology-place:happen_in rdf:resource="http://www.semanticweb.org/patriciapoveda/ontologies/2020/4/ontology-place.owl#Route1"/>
        <ontology-place:last rdf:resource="http://www.semanticweb.org/patriciapoveda/ontologies/2020/4/ontology-place.owl#TimeStop3"/>
    </owl:NamedIndividual>
    


    <!-- http://www.semanticweb.org/patriciapoveda/ontologies/2020/4/ontology-place.owl#TimeAlmacén1 -->

    <owl:NamedIndividual rdf:about="http://www.semanticweb.org/patriciapoveda/ontologies/2020/4/ontology-place.owl#TimeAlmacén1">
        <rdf:type rdf:resource="http://www.ontologydesignpatterns.org/cp/owl/timeinterval.owl#TimeInterval"/>
        <timeinterval:hasIntervalEndDate rdf:datatype="http://www.w3.org/2001/XMLSchema#string">20:00</timeinterval:hasIntervalEndDate>
        <timeinterval:hasIntervalStartDate rdf:datatype="http://www.w3.org/2001/XMLSchema#string">9:00</timeinterval:hasIntervalStartDate>
    </owl:NamedIndividual>
    


    <!-- http://www.semanticweb.org/patriciapoveda/ontologies/2020/4/ontology-place.owl#TimeCliente1 -->

    <owl:NamedIndividual rdf:about="http://www.semanticweb.org/patriciapoveda/ontologies/2020/4/ontology-place.owl#TimeCliente1">
        <rdf:type rdf:resource="http://www.ontologydesignpatterns.org/cp/owl/timeinterval.owl#TimeInterval"/>
        <timeinterval:hasIntervalEndDate rdf:datatype="http://www.w3.org/2001/XMLSchema#string">14:00</timeinterval:hasIntervalEndDate>
        <timeinterval:hasIntervalStartDate rdf:datatype="http://www.w3.org/2001/XMLSchema#string">10:00</timeinterval:hasIntervalStartDate>
    </owl:NamedIndividual>
    


    <!-- http://www.semanticweb.org/patriciapoveda/ontologies/2020/4/ontology-place.owl#TimeStop1 -->

    <owl:NamedIndividual rdf:about="http://www.semanticweb.org/patriciapoveda/ontologies/2020/4/ontology-place.owl#TimeStop1">
        <rdf:type rdf:resource="http://www.ontologydesignpatterns.org/cp/owl/timeinterval.owl#TimeInterval"/>
        <timeinterval:hasIntervalEndDate rdf:datatype="http://www.w3.org/2001/XMLSchema#string">11:00</timeinterval:hasIntervalEndDate>
        <timeinterval:hasIntervalStartDate rdf:datatype="http://www.w3.org/2001/XMLSchema#string">10:45</timeinterval:hasIntervalStartDate>
    </owl:NamedIndividual>
    


    <!-- http://www.semanticweb.org/patriciapoveda/ontologies/2020/4/ontology-place.owl#TimeStop2 -->

    <owl:NamedIndividual rdf:about="http://www.semanticweb.org/patriciapoveda/ontologies/2020/4/ontology-place.owl#TimeStop2">
        <rdf:type rdf:resource="http://www.ontologydesignpatterns.org/cp/owl/timeinterval.owl#TimeInterval"/>
        <timeinterval:hasIntervalEndDate rdf:datatype="http://www.w3.org/2001/XMLSchema#string"></timeinterval:hasIntervalEndDate>
        <timeinterval:hasIntervalStartDate rdf:datatype="http://www.w3.org/2001/XMLSchema#string">12:20</timeinterval:hasIntervalStartDate>
    </owl:NamedIndividual>
    


    <!-- http://www.semanticweb.org/patriciapoveda/ontologies/2020/4/ontology-place.owl#TimeStop3 -->

    <owl:NamedIndividual rdf:about="http://www.semanticweb.org/patriciapoveda/ontologies/2020/4/ontology-place.owl#TimeStop3">
        <rdf:type rdf:resource="http://www.ontologydesignpatterns.org/cp/owl/timeinterval.owl#TimeInterval"/>
        <timeinterval:hasIntervalEndDate rdf:datatype="http://www.w3.org/2001/XMLSchema#string">17:00</timeinterval:hasIntervalEndDate>
        <timeinterval:hasIntervalStartDate rdf:datatype="http://www.w3.org/2001/XMLSchema#string">16:00</timeinterval:hasIntervalStartDate>
    </owl:NamedIndividual>
    


    <!-- 
    ///////////////////////////////////////////////////////////////////////////////////////
    //
    // General axioms
    //
    ///////////////////////////////////////////////////////////////////////////////////////
     -->

    <rdf:Description>
        <rdf:type rdf:resource="http://www.w3.org/2002/07/owl#AllDisjointClasses"/>
        <owl:members rdf:parseType="Collection">
            <rdf:Description rdf:about="http://www.semanticweb.org/patriciapoveda/ontologies/2020/4/ontology-place.owl#Break_Stop"/>
            <rdf:Description rdf:about="http://www.semanticweb.org/patriciapoveda/ontologies/2020/4/ontology-place.owl#Download_Stop"/>
            <rdf:Description rdf:about="http://www.semanticweb.org/patriciapoveda/ontologies/2020/4/ontology-place.owl#Incidence_Stop"/>
            <rdf:Description rdf:about="http://www.semanticweb.org/patriciapoveda/ontologies/2020/4/ontology-place.owl#Lunch_Stop"/>
            <rdf:Description rdf:about="http://www.semanticweb.org/patriciapoveda/ontologies/2020/4/ontology-place.owl#Pick-up_Stop"/>
            <rdf:Description rdf:about="http://www.semanticweb.org/patriciapoveda/ontologies/2020/4/ontology-place.owl#Weighing"/>
        </owl:members>
    </rdf:Description>
    <rdf:Description>
        <rdf:type rdf:resource="http://www.w3.org/2002/07/owl#AllDisjointClasses"/>
        <owl:members rdf:parseType="Collection">
            <rdf:Description rdf:about="http://www.semanticweb.org/patriciapoveda/ontologies/2020/4/ontology-place.owl#Scheduling"/>
            <rdf:Description rdf:about="http://www.semanticweb.org/patriciapoveda/ontologies/2020/4/ontology-place.owl#Stop"/>
            <rdf:Description rdf:about="http://www.semanticweb.org/patriciapoveda/ontologies/2020/4/ontology-place.owl#Storage"/>
            <rdf:Description rdf:about="http://www.semanticweb.org/patriciapoveda/ontologies/2020/4/ontology-place.owl#Transport"/>
        </owl:members>
    </rdf:Description>
</rdf:RDF>



<!-- Generated by the OWL API (version 4.5.9.2019-02-01T07:24:44Z) https://github.com/owlcs/owlapi -->

